A complete instruction bigrammar.

x86model/Model/Decode.v
@@ -143,6 +143,17 @@ End X86_PARSER_ARG.
   Definition operand_t := User_t Operand_t.
   Definition reg_or_immed_t := User_t Reg_or_Immed_t.
   Definition fp_operand_t := User_t Fp_Operand_t.  
+  Definition i_instr1_t := User_t I_Instr1_t.
+  Definition i_instr2_t := User_t I_Instr2_t.
+  Definition i_instr3_t := User_t I_Instr3_t.
+  Definition i_instr4_t := User_t I_Instr4_t.
+  Definition i_instr5_t := User_t I_Instr5_t.
+  Definition i_instr6_t := User_t I_Instr6_t.
+  Definition f_instr1_t := User_t F_Instr1_t.
+  Definition f_instr2_t := User_t F_Instr2_t.
+  Definition m_instr_t := User_t M_Instr_t.
+  Definition s_instr1_t := User_t S_Instr1_t.
+  Definition s_instr2_t := User_t S_Instr2_t.
   Definition instruction_t := User_t Instruction_t.
   Definition control_register_t := User_t Control_Register_t.
   Definition debug_register_t := User_t Debug_Register_t.
@@ -4213,7 +4224,7 @@ End X86_PARSER_ARG.
     ast_env_nil.
   Hint Unfold MOVD_env : env_unfold_db.
 
-  Definition MOVD_d : wf_bigrammar (pair_t mmx_operand_t mmx_operand_t).
+  Definition MOVD_p : wf_bigrammar (pair_t mmx_operand_t mmx_operand_t).
     gen_ast_defs MOVD_env.
     refine (gr @ (mp: _ -> [|pair_t mmx_operand_t mmx_operand_t|])
                & (fun u =>
@@ -4229,7 +4240,7 @@ End X86_PARSER_ARG.
       destruct v as [d [mr r]]; destruct d; printable_tac; ins_ibr_sim.
   Defined.
 
-  Definition MOVQ_d : wf_bigrammar (pair_t mmx_operand_t mmx_operand_t).
+  Definition MOVQ_p : wf_bigrammar (pair_t mmx_operand_t mmx_operand_t).
     refine (("0000" $$ "1111" $$ "011" $$ anybit $ "1111" $$ modrm_mmx)
              @ (fun v: [|pair_t char_t (pair_t mmx_operand_t mmx_operand_t)|] =>
                   let (d,v1):=v in let (op1,op2) :=v1 in
@@ -4972,152 +4983,6 @@ End X86_PARSER_ARG.
   Definition SFENCE_p := "0000" $$ "1111" $$ "1010" $$ "1110" $$ "1111"
                                 $$ ! "1000".
 
-  (** ** Hierarchical instruction syntax *)
-  (* To solve the scalability problem *)
-
-  (* Definition instr_grammars_rep := *)
-  (*   INS_p :: OUTS_p :: MOVS_p :: LODS_p :: STOS_p :: RET_p :: nil. *)
-
-  (* Definition instr_grammars_lock_with_op_override :=  *)
-  (*   ADD_p true :: ADC_p true :: AND_p true :: NEG_p :: NOT_p :: OR_p true *)
-  (*   :: SBB_p true :: SUB_p true :: XOR_p true :: XCHG_p :: nil. *)
-
-  (* Definition instr_grammars_lock_no_op_override :=  *)
-  (*   ADD_p false :: ADC_p false :: AND_p false :: BTC_p :: BTR_p ::  *)
-  (*   BTS_p :: CMPXCHG_p :: DEC_p :: INC_p :: NEG_p :: NOT_p :: OR_p false *)
-  (*   :: SBB_p false :: SUB_p false :: XOR_p false :: XADD_p :: XCHG_p :: nil. *)
-
-  (* Definition instr_grammars_seg_with_op_override :=  *)
-  (*   CMP_p true ::  IMUL_p true :: MOV_p true :: TEST_p true :: nil. *)
-
-  (* Definition instr_grammars_seg_op_override :=  *)
-  (*   CDQ_p :: CMOVcc_p :: CWDE_p :: DIV_p :: IDIV_p ::  *)
-  (*   MOVSX_p :: MOVZX_p :: MUL_p :: NOP_p ::  *)
-  (*   ROL_p :: ROR_p :: SAR_p :: SHL_p :: SHLD_p :: SHR_p :: SHRD_p :: nil. *)
-
-  (* Definition instr_grammars_seg_override :=  *)
-  (*   AAA_p :: AAD_p :: AAM_p :: AAS_p :: CMP_p false :: *)
-  (*   ARPL_p :: BOUND_p :: BSF_p :: BSR_p :: BSWAP_p :: BT_p ::  *)
-  (*   CALL_p :: CLC_p :: CLD_p :: CLI_p :: CLTS_p :: CMC_p :: CPUID_p :: DAA_p :: DAS_p :: *)
-  (*   HLT_p :: IMUL_p false :: IN_p :: INTn_p :: INT_p :: INTO_p :: INVD_p :: INVLPG_p :: IRET_p :: Jcc_p :: JCXZ_p :: JMP_p ::  *)
-  (*   LAHF_p :: LAR_p :: LDS_p :: LEA_p :: LEAVE_p :: LES_p :: LFS_p :: LGDT_p :: LGS_p :: LIDT_p :: LLDT_p :: LMSW_p ::  *)
-  (*   LOOP_p :: LOOPZ_p :: LOOPNZ_p :: LSL_p :: LSS_p :: LTR_p :: MOV_p false :: MOVCR_p :: MOVDR_p ::  *)
-  (*   MOVSR_p :: MOVBE_p ::  OUT_p :: POP_p :: POPSR_p :: POPA_p :: POPF_p :: *)
-  (*   PUSH_p :: PUSHSR_p :: PUSHA_p :: PUSHF_p :: RCL_p :: RCR_p :: RDMSR_p :: RDPMC_p :: RDTSC_p :: RDTSCP_p ::  *)
-  (*   RSM_p :: SAHF_p :: SETcc_p :: SGDT_p :: SIDT_p :: SLDT_p :: SMSW_p :: STC_p :: STD_p :: STI_p ::  *)
-  (*   STR_p :: TEST_p false :: UD2_p :: VERR_p :: VERW_p :: WBINVD_p :: WRMSR_p :: XLAT_p :: 
-   floating point instrs
-     F2XM1_p :: *)
-  (*   FABS_p :: FADD_p :: FADDP_p :: FBLD_p :: FBSTP_p :: FCHS_p :: FCMOVcc_p :: FCOM_p :: FCOMP_p :: FCOMPP_p :: FCOMIP_p :: FCOS_p :: FDECSTP_p :: *)
-  (*   FDIV_p :: FDIVP_p :: FDIVR_p :: FDIVRP_p :: FFREE_p :: FIADD_p :: FICOM_p :: FICOMP_p :: FIDIV_p :: FIDIVR_p :: FILD_p :: FIMUL_p :: FINCSTP_p *)
-  (*   :: FIST_p :: FISTP_p :: FISUB_p :: FISUBR_p :: FLD_p :: FLD1_p :: FLDCW_p :: FLDENV_p :: FLDL2E_p :: FLDL2T_p :: FLDLG2_p :: FLDLN2_p *)
-  (*   :: FLDPI_p :: FLDZ_p :: FMUL_p :: FMULP_p :: FNCLEX_p :: FNINIT_p :: FNOP_p :: FNSAVE_p :: FNSTCW_p :: FNSTSW_p :: FPATAN_p :: FPREM_p :: FPREM1_p :: FPTAN_p :: FRNDINT_p :: FRSTOR_p :: (* FSAVE_p :: *)  *)
-  (*   FSCALE_p ::  *)
-  (*   FSIN_p :: FSINCOS_p :: FSQRT_p :: FST_p :: (* FSTCW_p :: *) FSTENV_p :: FSTP_p :: FSUB_p :: FSUBP_p :: FSUBR_p :: FSUBRP_p ::FTST_p :: *)
-  (*   FUCOM_p :: FUCOMP_p :: FUCOMPP_p :: FUCOMI_p :: FUCOMIP_p :: FXAM_p :: FXCH_p :: FXTRACT_p :: FYL2X_p :: FYL2XP1_p :: FWAIT_p ::  *)
-  (*   EMMS_p :: MOVD_p :: MOVQ_p :: PACKSSDW_p :: PACKSSWB_p :: PACKUSWB_p :: PADD_p :: PADDS_p :: PADDUS_p :: PAND_p :: PANDN_p :: PCMPEQ_p :: PCMPGT_p ::  *)
-  (*   PMADDWD_p :: PMULHUW_p :: PMULHW_p :: PMULLW_p :: POR_p :: PSLL_p :: PSRA_p :: PSRL_p :: PSUB_p :: PSUBS_p :: PSUBUS_p :: PUNPCKH_p :: PUNPCKL_p :: PXOR_p ::  *)
-  (*   ADDPS_p :: ADDSS_p :: ANDNPS_p :: ANDPS_p :: CMPPS_p :: CMPSS_p :: COMISS_p :: CVTPI2PS_p :: CVTPS2PI_p :: CVTSI2SS_p :: CVTSS2SI_p :: CVTTPS2PI_p :: CVTTSS2SI_p :: *)
-  (*   DIVPS_p :: DIVSS_p :: LDMXCSR_p :: MAXPS_p :: MAXSS_p :: MINPS_p :: MINSS_p :: MOVAPS_p :: MOVHLPS_p :: MOVLPS_p :: MOVMSKPS_p :: MOVSS_p :: MOVUPS_p :: MULPS_p :: *)
-  (*   MULSS_p :: ORPS_p :: RCPPS_p :: RCPSS_p :: RSQRTPS_p :: RSQRTSS_p :: SHUFPS_p :: SQRTPS_p :: SQRTSS_p :: STMXCSR_p :: SUBPS_p :: SUBSS_p :: UCOMISS_p :: UNPCKHPS_p :: *)
-  (*   UNPCKLPS_p :: XORPS_p :: PAVGB_p :: PEXTRW_p :: PINSRW_p :: PMAXSW_p :: PMAXUB_p :: PMINSW_p :: PMINUB_p :: PMOVMSKB_p :: PSADBW_p :: PSHUFW_p :: MASKMOVQ_p :: *)
-  (*   MOVNTPS_p :: MOVNTQ_p :: PREFETCHT0_p :: PREFETCHT1_p :: PREFETCHT2_p :: PREFETCHNTA_p :: SFENCE_p :: nil. *)
-
-
-  (** This set of integer instructions
-     - take no parameters
-     - take only the seg_override prefix *)
-  Inductive i_instr1 : Set :=
-  | I_AAA
-  | I_AAD 
-  | I_AAM 
-  | I_AAS 
-  | I_CLC 
-  | I_CLD 
-  | I_CLI 
-  | I_CLTS 
-  | I_CMC
-  | I_CPUID 
-  | I_DAA 
-  | I_DAS
-  | I_HLT  
-  | I_INT
-  | I_INTO
-  | I_INVD
-  | I_IRET
-  | I_LAHF
-  | I_LEAVE
-  | I_POPA 
-  | I_POPF
-  | I_PUSHA
-  | I_PUSHF
-  | I_RDMSR
-  | I_RDPMC
-  | I_RDTSC
-  | I_RDTSCP
-  | I_RSM
-  | I_SAHF
-  | I_STC
-  | I_STD
-  | I_STI
-  | I_UD2
-  | I_WBINVD
-  | I_WRMSR
-  | I_XLAT.
-
-  (** This set of integer instructions
-     - take some parameters
-     - take only the seg_override prefix *)
-  Inductive i_instr2 : Set :=
-  | I_ARPL (op1 op2:operand)
-  | I_BOUND (op1 op2:operand)
-  | I_BSF (op1 op2:operand)
-  | I_BSR (op1 op2:operand)
-  | I_BSWAP (r:register)
-  | I_BT (op1 op2:operand)
-  | I_CALL (near:bool)(absolute: bool)(op1:operand)(sel:option selector)
-  | I_IN (w:bool)(p: option port_number)
-  | I_INTn (it:interrupt_type)
-  | I_INVLPG (op1:operand)
-  | I_Jcc (ct:condition_type)(disp:int32)
-  | I_JCXZ (b:int8)
-  | I_JMP (near:bool)(absolute:bool)(op1: operand)(sel:option selector)
-  | I_LAR (op1 op2:operand)
-  | I_LDS (op1 op2:operand)
-  | I_LEA (op1 op2:operand)
-  | I_LES (op1 op2:operand)
-  | I_LFS (op1 op2:operand)
-  | I_LGDT (op1:operand)
-  | I_LGS (op1 op2:operand)
-  | I_LIDT (op1:operand)
-  | I_LLDT (op1:operand)
-  | I_LMSW (op1:operand)
-  | I_LOOP (disp:int8)
-  | I_LOOPZ (disp:int8)
-  | I_LOOPNZ (disp:int8)
-  | I_LSL  (op1 op2:operand)
-  | I_LSS (op1 op2:operand)
-  | I_LTR (op1:operand)
-  | I_MOVCR (direction:bool)(cr:control_register)(r:register)
-  | I_MOVDR (direction:bool)(dr:debug_register)(r:register)
-  | I_MOVSR (direction:bool)(sr:segment_register)(op1:operand)
-  | I_MOVBE (op1 op2:operand)
-  | I_OUT (w:bool)(p:option port_number)
-  | I_POP (op1:operand)
-  | I_POPSR (sr:segment_register)
-  | I_PUSH (w:bool)(op1:operand)
-  | I_PUSHSR (sr:segment_register)
-  | I_RCL (w:bool)(op1:operand)(ri:reg_or_immed)
-  | I_RCR (w:bool)(op1:operand)(ri:reg_or_immed)
-  | I_SETcc (ct:condition_type)(op1:operand)
-  | I_SGDT (op1:operand)
-  | I_SIDT (op1:operand)
-  | I_SLDT (op1:operand)
-  | I_SMSW (op1:operand)
-  | I_STR (op1:operand)
-  | I_VERR (op1:operand)
-  | I_VERW (op1:operand).
-
   (** ** Glue all individual instruction grammars together into one big
          grammar.  *)
 
@@ -5263,20 +5128,6 @@ End X86_PARSER_ARG.
       destruct op; destruct addr; parsable_tac.
   Defined.
 
-  (** this set of instructions can take prefixes in prefix_grammar_rep;
-      that is, in lock_or_rep, only rep can be used; we put RET in this
-      category because it turns out many binaries use "rep ret" to avoid the
-      branch prediction panelty in AMD processors; intel processor seems to
-      just ignore the rep prefix in "rep ret". *)
-  (* Definition instr_grammars_rep_env : AST_Env instruction_t := *)
-  (*   {0, INS_p, (fun v => INS v %% instruction_t)} ::: *)
-  (*   {1, OUTS_p, (fun v => OUTS v %% instruction_t)} ::: *)
-  (*   {2, MOVS_p, (fun v => MOVS v %% instruction_t)} ::: *)
-  (*   {3, LODS_p, (fun v => LODS v %% instruction_t)} ::: *)
-  (*   {4, STOS_p, (fun v => STOS v %% instruction_t)} ::: *)
-  (*   {5, RET_p, (fun v => RET (fst v) (snd v) %% instruction_t)} ::: *)
-  (*   ast_env_nil. *)
-
   Definition prefix_grammar_rep_or_repn : wf_bigrammar prefix_t.
     refine ((option_perm3 rep_or_repn_p segment_override_p op_override_p)
               @ (fun v => match v with (l, (s, op)) =>
@@ -5299,13 +5150,6 @@ End X86_PARSER_ARG.
     - destruct w as [l s op addr];
       destruct op; destruct addr; parsable_tac.
   Defined.
-
-  (** this set of instructions can take prefixes in prefix_grammar_repn;
-      that is, in lock_or_rep, either rep or repn can be used, but not lock *)
-  (* Definition instr_grammars_rep_or_repn_env : AST_Env instruction_t := *)
-  (*   {10, CMPS_p, (fun v => CMPS v %% instruction_t)} ::: *)
-  (*   {11, SCAS_p, (fun v => SCAS v %% instruction_t)} ::: *)
-  (*   ast_env_nil. *)
 
   Definition prefix_grammar_lock_with_op_override : wf_bigrammar prefix_t.
     refine ((option_perm3_variation lock_p segment_override_p op_override_p)
@@ -5335,35 +5179,6 @@ End X86_PARSER_ARG.
     subst pre; trivial.
   Qed.
 
-  (** Instructions that can take prefixes in
-     prefix_grammar_lock_with_op_override: in lock_or_rep, only lock can be
-     used; segment override is optional; op_override prefix *must* be used;
-     NEG, NOT, and XCHG appear in both instr_grammars_lock_with_op_override_env
-     and instr_grammars_lock_no_op_override_env since they allow op_override
-     prefix to be optional. *)
-  (* Definition instr_grammars_lock_with_op_override_env : AST_Env instruction_t := *)
-  (*   {20, ADC_p true, (fun v => match v with (b,(op1,op2)) => ADC b op1 op2 end *)
-  (*                         %% instruction_t)} ::: *)
-  (*   {21, ADD_p true, (fun v => match v with (b,(op1,op2)) => ADD b op1 op2 end *)
-  (*                         %% instruction_t)} ::: *)
-  (*   {22, AND_p true, (fun v => match v with (b,(op1,op2)) => AND b op1 op2 end *)
-  (*                         %% instruction_t)} ::: *)
-  (*   {23, NEG_p, (fun v => match v with (b,op) => NEG b op end *)
-  (*                         %% instruction_t)} ::: *)
-  (*   {24, NOT_p, (fun v => match v with (b,op) => NOT b op end *)
-  (*                         %% instruction_t)} ::: *)
-  (*   {25, OR_p true, (fun v => match v with (b,(op1,op2)) => OR b op1 op2 end *)
-  (*                         %% instruction_t)} ::: *)
-  (*   {26, SBB_p true, (fun v => match v with (b,(op1,op2)) => SBB b op1 op2 end *)
-  (*                         %% instruction_t)} ::: *)
-  (*   {27, SUB_p true, (fun v => match v with (b,(op1,op2)) => SUB b op1 op2 end *)
-  (*                         %% instruction_t)} ::: *)
-  (*   {28, XCHG_p, (fun v => match v with (b,(op1,op2)) => XCHG b op1 op2 end *)
-  (*                         %% instruction_t)} ::: *)
-  (*   {29, XOR_p true, (fun v => match v with (b,(op1,op2)) => XOR b op1 op2 end *)
-  (*                         %% instruction_t)} ::: *)
-  (*   ast_env_nil. *)
-
   Definition prefix_grammar_lock_no_op_override : wf_bigrammar prefix_t.
     refine ((option_perm2 lock_p segment_override_p)
               @ (fun v => match v with (l, s) =>
@@ -5385,47 +5200,6 @@ End X86_PARSER_ARG.
     ibr_prover. subst pre; trivial. 
   Qed.
 
-  (** Instructions that can take prefixes in
-     prefix_grammar_lock_no_op_override; that is, in lock_or_rep, only lock
-     can be used; segment override is optional; and op_override prefix
-     *must not* be used *)
-  (* Definition instr_grammars_lock_no_op_override_env : AST_Env instruction_t := *)
-  (*   {30, ADC_p false, (fun v => match v with (b,(op1,op2)) => ADC b op1 op2 end *)
-  (*                         %% instruction_t)} ::: *)
-  (*   {31, ADD_p false, (fun v => match v with (b,(op1,op2)) => ADD b op1 op2 end *)
-  (*                         %% instruction_t)} ::: *)
-  (*   {32, AND_p false, (fun v => match v with (b,(op1,op2)) => AND b op1 op2 end *)
-  (*                         %% instruction_t)} ::: *)
-  (*   {33, BTC_p, (fun v => match v with (op1,op2) => BTC op1 op2 end *)
-  (*                         %% instruction_t)} ::: *)
-  (*   {34, BTR_p, (fun v => match v with (op1,op2) => BTR op1 op2 end *)
-  (*                         %% instruction_t)} ::: *)
-  (*   {35, BTS_p, (fun v => match v with (op1,op2) => BTS op1 op2 end *)
-  (*                         %% instruction_t)} ::: *)
-  (*   {36, CMPXCHG_p, (fun v => match v with (b,(op1,op2)) => CMPXCHG b op1 op2 end *)
-  (*                         %% instruction_t)} ::: *)
-  (*   {37, DEC_p, (fun v => match v with (b,op) => DEC b op end *)
-  (*                         %% instruction_t)} ::: *)
-  (*   {38, INC_p, (fun v => match v with (b,op) => INC b op end *)
-  (*                         %% instruction_t)} ::: *)
-  (*   {39, NEG_p, (fun v => match v with (b,op) => NEG b op end *)
-  (*                         %% instruction_t)} ::: *)
-  (*   {40, NOT_p, (fun v => match v with (b,op) => NOT b op end *)
-  (*                         %% instruction_t)} ::: *)
-  (*   {41, OR_p false, (fun v => match v with (b,(op1,op2)) => OR b op1 op2 end *)
-  (*                         %% instruction_t)} ::: *)
-  (*   {42, SBB_p false, (fun v => match v with (b,(op1,op2)) => SBB b op1 op2 end *)
-  (*                         %% instruction_t)} ::: *)
-  (*   {43, SUB_p false, (fun v => match v with (b,(op1,op2)) => SUB b op1 op2 end *)
-  (*                         %% instruction_t)} ::: *)
-  (*   {44, XADD_p, (fun v => match v with (b,(op1,op2)) => XADD b op1 op2 end *)
-  (*                         %% instruction_t)} ::: *)
-  (*   {45, XCHG_p, (fun v => match v with (b,(op1,op2)) => XCHG b op1 op2 end *)
-  (*                         %% instruction_t)} ::: *)
-  (*   {46, XOR_p false, (fun v => match v with (b,(op1,op2)) => XOR b op1 op2 end *)
-  (*                         %% instruction_t)} ::: *)
-  (*   ast_env_nil. *)
-
   Definition prefix_grammar_seg_with_op_override: wf_bigrammar prefix_t. 
     refine ((option_perm2_variation segment_override_p op_override_p)
               @ (fun v => match v with (s, op) =>
@@ -5439,22 +5213,6 @@ End X86_PARSER_ARG.
       ins_invertible_tac.
     - destruct w as [l s op addr]; destruct l; destruct addr; parsable_tac.
   Defined.
-
-  (* this set of instructions can take prefixes in 
-     prefix_grammar_seg_with_op_override;
-     that is, it cannot take a lock_or_rep prefix, must take op_override
-     prefix, can optionally take segment-override prefix *)
-  (* Definition instr_grammars_seg_with_op_override_env : AST_Env instruction_t := *)
-  (*   {50, CMP_p true, (fun v => match v with (b,(op1,op2)) => CMP b op1 op2 end *)
-  (*                         %% instruction_t)} ::: *)
-  (*   {51, IMUL_p true, (fun v => match v with (b,(op1,(opopt,iopt))) => *)
-  (*                                  IMUL b op1 opopt iopt end *)
-  (*                         %% instruction_t)} ::: *)
-  (*   {52, MOV_p true, (fun v => match v with (b,(op1,op2)) => MOV b op1 op2 end *)
-  (*                         %% instruction_t)} ::: *)
-  (*   {53, TEST_p true, (fun v => match v with (b,(op1,op2)) => TEST b op1 op2 end *)
-  (*                         %% instruction_t)} ::: *)
-  (*   ast_env_nil. *)
 
   Definition prefix_grammar_seg_op_override: wf_bigrammar prefix_t. 
     refine ((option_perm2 segment_override_p op_override_p)
@@ -5517,7 +5275,7 @@ End X86_PARSER_ARG.
   (*   ast_env_nil. *)
 
   (* only allows seg override prefix *)
-  Definition prefix_grammar_seg_override_only : wf_bigrammar prefix_t.
+  Definition prefix_grammar_only_seg_override : wf_bigrammar prefix_t.
     refine ((option_perm segment_override_p)
               @ (fun s => mkPrefix None s false false %% prefix_t)
               & (fun u => 
@@ -5531,26 +5289,1952 @@ End X86_PARSER_ARG.
       destruct op; destruct addr; destruct l; parsable_tac.
   Defined.
 
-  (* this set of instructions can take only the seg_override prefix *)
-  Definition instr_grammars_seg_override : AST_Env instruction_t :=
-    {100, AAA_p, (fun v => AAA %% instruction_t)} :::
-    {101, AAD_p, (fun v => AAD %% instruction_t)} :::
-    {102, AAM_p, (fun v => AAM %% instruction_t)} :::
-    {103, AAS_p, (fun v => AAS %% instruction_t)} :::
-    {104, ARPL_p, (fun v => match v with (op1,op2) => ARPL op1 op2 end
-                          %% instruction_t)} :::
-    {105, BOUND_p, (fun v => match v with (op1,op2) => BOUND op1 op2 end
-                          %% instruction_t)} :::
-    {106, BSF_p, (fun v => match v with (op1,op2) => BSF op1 op2 end
-                          %% instruction_t)} :::
-    {107, BSR_p, (fun v => match v with (op1,op2) => BSR op1 op2 end
-                          %% instruction_t)} :::
-    {108, BSWAP_p, (fun r => BSWAP r %% instruction_t)} :::
-    {109, BT_p, (fun v => match v with (op1,op2) => BT op1 op2 end
-                          %% instruction_t)} :::
-    {110, CMP_p false, (fun v => match v with (b,(op1,op2)) => CMP b op1 op2 end
-                          %% instruction_t)} :::
+  Lemma seg_with_op_override_rng_inv pre: 
+    in_bigrammar_rng (` prefix_grammar_seg_with_op_override) pre ->
+    op_override pre = true.
+  Proof. unfold prefix_grammar_seg_with_op_override; intros.
+    ibr_prover.
+    match goal with
+      | [H:in_bigrammar_rng (` (option_perm2_variation _ _)) (_,_) |- _] =>
+        rewrite <- option_perm2_variation_rng in H; destruct H as [_ H];
+        apply op_override_p_rng_inv in H
+    end.
+    subst pre; trivial.
+  Qed.
+
+  Lemma only_seg_override_rng_inv pre: 
+    in_bigrammar_rng (` prefix_grammar_only_seg_override) pre ->
+    op_override pre = false.
+  Proof. unfold prefix_grammar_only_seg_override; intros.
+    ibr_prover.
+    subst pre; trivial.
+  Qed.
+
+  Definition i_instr1_env : AST_Env i_instr1_t := 
+    {0, AAA_p, (fun v => I_AAA %% i_instr1_t)} :::
+    {1, AAD_p, (fun v => I_AAD %% i_instr1_t)} :::
+    {2, AAM_p, (fun v => I_AAM %% i_instr1_t)} :::
+    {3, AAS_p, (fun v => I_AAS %% i_instr1_t)} :::
+    {4, CLC_p, (fun v => I_CLC %% i_instr1_t)} :::
+    {5, CLD_p, (fun v => I_CLD %% i_instr1_t)} :::
+    {6, CLI_p, (fun v => I_CLI %% i_instr1_t)} :::
+    {7, CLTS_p, (fun v => I_CLTS %% i_instr1_t)} :::
+    {8, CMC_p, (fun v => I_CMC %% i_instr1_t)} :::
+    {9, CPUID_p, (fun v => I_CPUID %% i_instr1_t)} :::
+    {10, DAA_p, (fun v => I_DAA %% i_instr1_t)} :::
+    {11, DAS_p, (fun v => I_DAS %% i_instr1_t)} :::
+    {12, HLT_p, (fun v => I_HLT %% i_instr1_t)} :::
+    {13, INT_p, (fun v => I_INT %% i_instr1_t)} :::
+    {14, INTO_p, (fun v => I_INTO %% i_instr1_t)} :::
+    {15, INVD_p, (fun v => I_INVD %% i_instr1_t)} :::
+    {16, IRET_p, (fun v => I_IRET %% i_instr1_t)} :::
+    {17, LAHF_p, (fun v => I_LAHF %% i_instr1_t)} :::
+    {18, LEAVE_p, (fun v => I_LEAVE %% i_instr1_t)} :::
+    {19, POPA_p, (fun v => I_POPA %% i_instr1_t)} :::
+    {20, POPF_p, (fun v => I_POPF %% i_instr1_t)} :::
+    {21, PUSHA_p, (fun v => I_PUSHA %% i_instr1_t)} :::
+    {22, PUSHF_p, (fun v => I_PUSHF %% i_instr1_t)} :::
+    {23, RDMSR_p, (fun v => I_RDMSR %% i_instr1_t)} :::
+    {24, RDPMC_p, (fun v => I_RDPMC %% i_instr1_t)} :::
+    {25, RDTSC_p, (fun v => I_RDTSC %% i_instr1_t)} :::
+    {26, RDTSCP_p, (fun v => I_RDTSCP %% i_instr1_t)} :::
+    {27, RSM_p, (fun v => I_RSM %% i_instr1_t)} :::
+    {28, SAHF_p, (fun v => I_SAHF %% i_instr1_t)} :::
+    {29, STC_p, (fun v => I_STC %% i_instr1_t)} :::
+    {30, STD_p, (fun v => I_STD %% i_instr1_t)} :::
+    {31, STI_p, (fun v => I_STI %% i_instr1_t)} :::
+    {32, UD2_p, (fun v => I_UD2 %% i_instr1_t)} :::
+    {33, WBINVD_p, (fun v => I_WBINVD %% i_instr1_t)} :::
+    {34, WRMSR_p, (fun v => I_WRMSR %% i_instr1_t)} :::
+    {35, XLAT_p, (fun v => I_XLAT %% i_instr1_t)} :::
     ast_env_nil.
+  Hint Unfold i_instr1_env: env_unfold_db.
+
+  Definition i_instr1_p : wf_bigrammar i_instr1_t.
+    Time gen_ast_defs i_instr1_env.
+    refine (gr @ (mp: _ -> [|i_instr1_t|])
+               & (fun u =>
+                    match u with
+                      | I_AAA => case0 ()
+                      | I_AAD => case1 ()
+                      | I_AAM => case2 ()
+                      | I_AAS => case3 ()
+                      | I_CLC => case4 ()
+                      | I_CLD => case5 ()
+                      | I_CLI => case6 ()
+                      | I_CLTS => case7 ()
+                      | I_CMC => case8 ()
+                      | I_CPUID => case9 ()
+                      | I_DAA => case10 ()
+                      | I_DAS => case11 ()
+                      | I_HLT => case12 ()
+                      | I_INT => case13 ()
+                      | I_INTO => case14 ()
+                      | I_INVD => case15 ()
+                      | I_IRET => case16 ()
+                      | I_LAHF => case17 ()
+                      | I_LEAVE => case18 ()
+                      | I_POPA => case19 ()
+                      | I_POPF => case20 ()
+                      | I_PUSHA => case21 ()
+                      | I_PUSHF => case22 ()
+                      | I_RDMSR => case23 ()
+                      | I_RDPMC => case24 ()
+                      | I_RDTSC => case25 ()
+                      | I_RDTSCP => case26 ()
+                      | I_RSM => case27 ()
+                      | I_SAHF => case28 ()
+                      | I_STC => case29 ()
+                      | I_STD => case30 ()
+                      | I_STI => case31 ()
+                      | I_UD2 => case32 ()
+                      | I_WBINVD => case33 ()
+                      | I_WRMSR => case34 ()
+                      | I_XLAT => case35 ()
+                    end)
+               & _); clear_ast_defs; invertible_tac.
+     - Time abstract (destruct w; parsable_tac).
+  Defined.
+
+  Definition i_instr2_env : AST_Env i_instr2_t := 
+    {0, ARPL_p, (fun v => match v with (op1,op2) => I_ARPL op1 op2
+                          end %% i_instr2_t)} :::
+    {1, BOUND_p, (fun v => match v with (op1,op2) => I_BOUND op1 op2
+                          end %% i_instr2_t)} :::
+    {2, BSF_p, (fun v => match v with (op1,op2) => I_BSF op1 op2
+                          end %% i_instr2_t)} :::
+    {3, BSR_p, (fun v => match v with (op1,op2) => I_BSR op1 op2
+                          end %% i_instr2_t)} :::
+    {4, BSWAP_p, (fun r => I_BSWAP r %% i_instr2_t)} :::
+    {5, BT_p, (fun v => match v with (op1,op2) => I_BT op1 op2
+                          end %% i_instr2_t)} :::
+    {6, CALL_p, (fun v => match v with
+                              (near,(abs,(op1,sel))) => I_CALL near abs op1 sel
+                          end %% i_instr2_t)} :::
+    {7, IN_p, (fun v => match v with (w,p) => I_IN w p
+                          end %% i_instr2_t)} :::
+    {8, INTn_p, (fun it => I_INTn it %% i_instr2_t)} :::
+    {9, INVLPG_p, (fun op => I_INVLPG op %% i_instr2_t)} :::
+    {10, Jcc_p, (fun v => match v with (ct,disp) => I_Jcc ct disp
+                          end %% i_instr2_t)} :::
+    {11, JCXZ_p, (fun b => I_JCXZ b %% i_instr2_t)} :::
+    {12, JMP_p, (fun v => match v with
+                              (near,(abs,(op1,sel))) => I_JMP near abs op1 sel
+                          end %% i_instr2_t)} :::
+    {13, LAR_p, (fun v => match v with (op1,op2) => I_LAR op1 op2
+                          end %% i_instr2_t)} :::
+    {14, LDS_p, (fun v => match v with (op1,op2) => I_LDS op1 op2
+                          end %% i_instr2_t)} :::
+    {15, LEA_p, (fun v => match v with (op1,op2) => I_LEA op1 op2
+                          end %% i_instr2_t)} :::
+    {16, LES_p, (fun v => match v with (op1,op2) => I_LES op1 op2
+                          end %% i_instr2_t)} :::
+    {17, LFS_p, (fun v => match v with (op1,op2) => I_LFS op1 op2
+                          end %% i_instr2_t)} :::
+    {18, LGDT_p, (fun op => I_LGDT op %% i_instr2_t)} :::
+    {19, LGS_p, (fun v => match v with (op1,op2) => I_LGS op1 op2
+                          end %% i_instr2_t)} :::
+    {20, LIDT_p, (fun op => I_LIDT op %% i_instr2_t)} :::
+    {21, LLDT_p, (fun op => I_LLDT op %% i_instr2_t)} :::
+    {22, LMSW_p, (fun op => I_LMSW op %% i_instr2_t)} :::
+    {23, LOOP_p, (fun di => I_LOOP di %% i_instr2_t)} :::
+    {24, LOOPZ_p, (fun di => I_LOOPZ di %% i_instr2_t)} :::
+    {25, LOOPNZ_p, (fun di => I_LOOPNZ di %% i_instr2_t)} :::
+    {26, LSL_p, (fun v => match v with (op1,op2) => I_LSL op1 op2
+                          end %% i_instr2_t)} :::
+    {27, LSS_p, (fun v => match v with (op1,op2) => I_LSS op1 op2
+                          end %% i_instr2_t)} :::
+    {28, LTR_p, (fun op => I_LTR op %% i_instr2_t)} :::
+    ast_env_nil.
+  Hint Unfold i_instr2_env: env_unfold_db.
+
+  Definition i_instr2_p : wf_bigrammar i_instr2_t.
+    gen_ast_defs i_instr2_env.
+    refine (gr @ (mp: _ -> [|i_instr2_t|])
+               & (fun u =>
+                    match u with
+                      | I_ARPL op1 op2 => case0 (op1,op2)
+                      | I_BOUND op1 op2 => case1 (op1,op2)
+                      | I_BSF op1 op2 => case2 (op1,op2)
+                      | I_BSR op1 op2 => case3 (op1,op2)
+                      | I_BSWAP r => case4 r
+                      | I_BT op1 op2 => case5 (op1,op2)
+                      | I_CALL near abs op1 sel => case6 (near,(abs,(op1,sel)))
+                      | I_IN w p => case7 (w,p)
+                      | I_INTn it => case8 it
+                      | I_INVLPG op => case9 op
+                      | I_Jcc ct disp => case10 (ct,disp)
+                      | I_JCXZ b => case11 b
+                      | I_JMP near abs op1 sel => case12 (near,(abs,(op1,sel)))
+                      | I_LAR op1 op2 => case13 (op1,op2)
+                      | I_LDS op1 op2 => case14 (op1,op2)
+                      | I_LEA op1 op2 => case15 (op1,op2)
+                      | I_LES op1 op2 => case16 (op1,op2)
+                      | I_LFS op1 op2 => case17 (op1,op2)
+                      | I_LGDT op1 => case18 op1
+                      | I_LGS op1 op2 => case19 (op1,op2)
+                      | I_LIDT op1 => case20 op1
+                      | I_LLDT op1 => case21 op1
+                      | I_LMSW op1 => case22 op1
+                      | I_LOOP disp => case23 disp
+                      | I_LOOPZ disp => case24 disp
+                      | I_LOOPNZ disp => case25 disp
+                      | I_LSL op1 op2 => case26 (op1,op2)
+                      | I_LSS op1 op2 => case27 (op1,op2)
+                      | I_LTR op1 => case28 op1
+                    end)
+               & _); clear_ast_defs;
+    unfold invertible; split; [unfold printable | unfold parsable]; 
+    compute [snd fst]; intros.
+    - repeat match goal with
+               | [v: [| Sum_t _ _ |] |- _ ] => case v as [v | v]
+               | [v: [| unit_t |] |- _] => destruct v
+               | [v:[|pair_t _ _|] |- _] => destruct v
+             end; abstract printable_tac.
+    - abstract (destruct w; parsable_tac).
+  Defined.
+
+  Definition i_instr3_env : AST_Env i_instr3_t := 
+    {0, MOVCR_p, (fun v => match v with (d,(cr,r)) => I_MOVCR d cr r
+                          end %% i_instr3_t)} :::
+    {1, MOVDR_p, (fun v => match v with (d,(cr,r)) => I_MOVDR d cr r
+                          end %% i_instr3_t)} :::
+    {2, MOVSR_p, (fun v => match v with (d,(cr,r)) => I_MOVSR d cr r
+                          end %% i_instr3_t)} :::
+    {3, MOVBE_p, (fun v => match v with (op1,op2) => I_MOVBE op1 op2
+                          end %% i_instr3_t)} :::
+    {4, OUT_p, (fun v => match v with (w,p) => I_OUT w p
+                          end %% i_instr3_t)} :::
+    {5, POP_p, (fun op => I_POP op %% i_instr3_t)} :::
+    {6, POPSR_p, (fun sr => I_POPSR sr %% i_instr3_t)} :::
+    {7, PUSH_p, (fun v => match v with (w,op1) => I_PUSH w op1
+                          end %% i_instr3_t)} :::
+    {8, PUSHSR_p, (fun sr => I_PUSHSR sr %% i_instr3_t)} :::
+    {9, RCL_p, (fun v => match v with (w,(op1,ri)) => I_RCL w op1 ri
+                          end %% i_instr3_t)} :::
+    {10, RCR_p, (fun v => match v with (w,(op1,ri)) => I_RCR w op1 ri
+                          end %% i_instr3_t)} :::
+    {11, SETcc_p, (fun v => match v with (ct,op1) => I_SETcc ct op1
+                          end %% i_instr3_t)} :::
+    {12, SGDT_p, (fun op => I_SGDT op %% i_instr3_t)} :::
+    {13, SIDT_p, (fun op => I_SIDT op %% i_instr3_t)} :::
+    {14, SLDT_p, (fun op => I_SLDT op %% i_instr3_t)} :::
+    {15, SMSW_p, (fun op => I_SMSW op %% i_instr3_t)} :::
+    {16, STR_p, (fun op => I_STR op %% i_instr3_t)} :::
+    {17, VERR_p, (fun op => I_VERR op %% i_instr3_t)} :::
+    {18, VERW_p, (fun op => I_VERW op %% i_instr3_t)} :::
+    ast_env_nil.
+  Hint Unfold i_instr3_env: env_unfold_db.
+
+  Definition i_instr3_p : wf_bigrammar i_instr3_t.
+    gen_ast_defs i_instr3_env.
+    refine (gr @ (mp: _ -> [|i_instr3_t|])
+               & (fun u =>
+                    match u with
+                      | I_MOVCR d cr r => case0 (d,(cr,r))
+                      | I_MOVDR d cr r => case1 (d,(cr,r))
+                      | I_MOVSR d cr r => case2 (d,(cr,r))
+                      | I_MOVBE op1 op2 => case3 (op1,op2)
+                      | I_OUT w p => case4 (w,p)
+                      | I_POP op => case5 op
+                      | I_POPSR sr => case6 sr
+                      | I_PUSH w op1 => case7 (w,op1)
+                      | I_PUSHSR sr => case8 sr
+                      | I_RCL w op1 ri => case9 (w,(op1,ri))
+                      | I_RCR w op1 ri => case10 (w,(op1,ri))
+                      | I_SETcc ct op1 => case11 (ct,op1)
+                      | I_SGDT op => case12 op
+                      | I_SIDT op => case13 op
+                      | I_SLDT op => case14 op
+                      | I_SMSW op => case15 op
+                      | I_STR op => case16 op
+                      | I_VERR op => case17 op 
+                      | I_VERW op => case18 op 
+                    end)
+               & _); clear_ast_defs;
+    unfold invertible; split; [unfold printable | unfold parsable]; 
+    compute [snd fst]; intros.
+    - repeat match goal with
+               | [v: [| Sum_t _ _ |] |- _ ] => case v as [v | v]
+               | [v: [| unit_t |] |- _] => destruct v
+               | [v:[|pair_t _ _|] |- _] => destruct v
+             end; abstract printable_tac.
+    - abstract (destruct w; parsable_tac).
+  Defined.
+
+  (** this set of instructions can take prefixes in prefix_grammar_rep;
+      that is, in lock_or_rep, only rep can be used; we put RET in this
+      category because it turns out many binaries use "rep ret" to avoid the
+      branch prediction panelty in AMD processors; intel processor seems to
+      just ignore the rep prefix in "rep ret". *)
+  Definition prefix_grammar_rep_env : AST_Env i_instr4_t := 
+    {0, INS_p, (fun v => I_INS v %% i_instr4_t)} :::
+    {1, OUTS_p, (fun v => I_OUTS v %% i_instr4_t)} :::
+    {2, MOVS_p, (fun v => I_MOVS v %% i_instr4_t)} :::
+    {3, LODS_p, (fun v => I_LODS v %% i_instr4_t)} :::
+    {4, STOS_p, (fun v => I_STOS v %% i_instr4_t)} :::
+    {5, RET_p, (fun v => I_RET (fst v) (snd v) %% i_instr4_t)} :::
+    ast_env_nil.
+     
+  (** this set of instructions can take prefixes in prefix_grammar_repn;
+      that is, in lock_or_rep, either rep or repn can be used, but not lock *)
+  Definition prefix_grammar_rep_or_repn_env : AST_Env i_instr4_t :=
+    {10, CMPS_p, (fun v => I_CMPS v %% i_instr4_t)} :::
+    {11, SCAS_p, (fun v => I_SCAS v %% i_instr4_t)} :::
+    ast_env_nil.
+
+  Hint Unfold prefix_grammar_rep_env 
+       prefix_grammar_rep_or_repn_env: env_unfold_db.
+
+ (* todo: maybe better names for hierachical instr syntax *)
+
+  Definition i_instr4_grammar_env' := 
+    (ast_env_cat prefix_grammar_rep prefix_grammar_rep_env)
+      +++
+    (ast_env_cat prefix_grammar_rep_or_repn 
+       prefix_grammar_rep_or_repn_env).
+
+  Definition i_instr4_grammar_env : AST_Env (pair_t prefix_t i_instr4_t).
+    let ige := eval cbv beta
+                    delta [i_instr4_grammar_env' prefix_grammar_rep_env
+                           prefix_grammar_rep_or_repn_env
+                           ast_env_app ast_env_cat]
+                    iota zeta 
+               in i_instr4_grammar_env' in
+    exact(ige).
+  Defined.
+
+  Definition i_instr4_grammar_type : type.
+    let ige := eval unfold i_instr4_grammar_env in i_instr4_grammar_env in
+    let t:=gen_ast_type ige in exact(t).
+  Defined.
+
+  Definition from_instr4 (u:prefix * i_instr4) : option [|i_instr4_grammar_type|].
+    intro.
+    refine (match snd u with
+              | I_INS a1 => _
+              | I_OUTS a1 => _
+              | I_MOVS a1 => _
+              | I_LODS a1 => _ 
+              | I_STOS a1 => _ 
+              | I_RET a1 a2 => _
+              | I_CMPS a1 => _
+              | I_SCAS a1 => _ 
+            end).
+    Local Ltac gen4 lbl u arg :=
+      let ige := eval unfold i_instr4_grammar_env
+                 in i_instr4_grammar_env in
+      let t := eval unfold i_instr4_grammar_type
+                 in i_instr4_grammar_type in
+      let f:=gen_rev_case_lbl lbl ige t in
+      let f1 := eval simpl in f in
+      exact (Some (f1 (fst u, arg))).
+    * (* I_INS *) gen4 0 u a1.
+    * (* I_OUTS *) gen4 1 u a1.
+    * (* I_MOVS *) gen4 2 u a1.
+    * (* I_LODS *) gen4 3 u a1.
+    * (* I_STOS *) gen4 4 u a1.
+    * (* I_RET *) gen4 5 u (a1,a2).
+    * (* I_CMPS *) gen4 10 u a1.
+    * (* I_SCAS *) gen4 11 u a1.
+  Defined.
+
+  (* todo: move earlier; better names *)
+  Local Ltac instr_printable := 
+    repeat match goal with
+             | [v: [| Sum_t _ _ |] |- _ ] => case v as [v | v]
+             | [v: [| unit_t |] |- _] => destruct v
+             | [v:[|pair_t _ _|] |- _] => destruct v
+           end;
+    try (match goal with
+           | [ |- exists v', ?c = Some v' /\ _] => 
+             match c with
+               | Some ?v =>
+                 exists v; split; trivial
+               | if op_override _ then Some ?v1 else Some ?v2 =>
+                 ibr_prover;
+                 match goal with
+                   | [ H: in_bigrammar_rng
+                            (` prefix_grammar_lock_with_op_override) ?pre |- _] =>
+                     assert (H2: op_override pre = true) by
+                         (apply lock_with_op_override_rng_inv; trivial);
+                     rewrite H2;
+                     exists v1; split; ibr_prover
+                   | [ H: in_bigrammar_rng
+                            (` prefix_grammar_lock_no_op_override) ?pre |- _] =>
+                     assert (H2: op_override pre = false) by
+                         (apply lock_no_op_override_rng_inv; trivial);
+                     rewrite H2;
+                     exists v2; split; ibr_prover
+                   | [ H: in_bigrammar_rng
+                            (` prefix_grammar_seg_with_op_override) ?pre |- _] =>
+                     assert (H2: op_override pre = true) by
+                         (apply seg_with_op_override_rng_inv; trivial);
+                     rewrite H2;
+                     exists v1; split; ibr_prover
+                   | [ H: in_bigrammar_rng
+                            (` prefix_grammar_only_seg_override) ?pre |- _] =>
+                     assert (H2: op_override pre = false) by
+                         (apply only_seg_override_rng_inv; trivial);
+                     rewrite H2;
+                     exists v2; split; ibr_prover
+                 end
+             end
+        end).
+
+  Local Ltac ins_parsable := 
+    match goal with
+      | [H: ?c = Some _ |- _] => 
+        match c with
+          | None => discriminate H
+          | Some _ => inversion H; clear H; subst; trivial
+          | if op_override ?p then Some _ else Some _ => 
+            destruct (op_override p);
+              inversion H; clear H; subst; trivial
+        end
+    end.
+
+  Definition i_instr4_grammar : wf_bigrammar (pair_t prefix_t i_instr4_t).
+    let ige := eval unfold i_instr4_grammar_env in i_instr4_grammar_env in
+    let g := gen_ast_grammar ige in pose (gr:=g);
+    let m := gen_ast_map ige in pose (mp:=m).
+    Time refine (gr @ (mp: _ -> [|pair_t prefix_t i_instr4_t|])
+                 & from_instr4
+                 & _); clear_ast_defs; unfold from_instr4;
+    unfold invertible; split; [unfold printable | unfold parsable];
+    compute [snd fst]; intros.
+    - abstract instr_printable.
+    - abstract (destruct w as [p ins]; destruct ins; ins_parsable).
+  Defined.
+
+  (** Instructions that can take prefixes in
+     prefix_grammar_lock_with_op_override: in lock_or_rep, only lock can be
+     used; segment override is optional; op_override prefix *must* be used;
+     NEG, NOT, and XCHG appear in both instr_grammars_lock_with_op_override_env
+     and instr_grammars_lock_no_op_override_env since they allow op_override
+     prefix to be optional. *)
+  Definition prefix_lock_with_op_override_env : AST_Env i_instr5_t :=
+    {0, ADC_p true, (fun v => match v with (b,(op1,op2)) => I_ADC b op1 op2 end
+                          %% i_instr5_t)} :::
+    {1, ADD_p true, (fun v => match v with (b,(op1,op2)) => I_ADD b op1 op2 end
+                          %% i_instr5_t)} :::
+    {2, AND_p true, (fun v => match v with (b,(op1,op2)) => I_AND b op1 op2 end
+                          %% i_instr5_t)} :::
+    {3, NEG_p, (fun v => match v with (b,op) => I_NEG b op end
+                          %% i_instr5_t)} :::
+    {4, NOT_p, (fun v => match v with (b,op) => I_NOT b op end
+                          %% i_instr5_t)} :::
+    {5, OR_p true, (fun v => match v with (b,(op1,op2)) => I_OR b op1 op2 end
+                          %% i_instr5_t)} :::
+    {6, SBB_p true, (fun v => match v with (b,(op1,op2)) => I_SBB b op1 op2 end
+                          %% i_instr5_t)} :::
+    {7, SUB_p true, (fun v => match v with (b,(op1,op2)) => I_SUB b op1 op2 end
+                          %% i_instr5_t)} :::
+    {8, XCHG_p, (fun v => match v with (b,(op1,op2)) => I_XCHG b op1 op2 end
+                          %% i_instr5_t)} :::
+    {9, XOR_p true, (fun v => match v with (b,(op1,op2)) => I_XOR b op1 op2 end
+                          %% i_instr5_t)} :::
+    ast_env_nil.
+
+  (** Instructions that can take prefixes in
+     prefix_grammar_lock_no_op_override; that is, in lock_or_rep, only lock
+     can be used; segment override is optional; and op_override prefix
+     *must not* be used *)
+  Definition prefix_lock_no_op_override_env : AST_Env i_instr5_t :=
+    {20, ADC_p false, (fun v => match v with (b,(op1,op2)) => I_ADC b op1 op2 end
+                          %% i_instr5_t)} :::
+    {21, ADD_p false, (fun v => match v with (b,(op1,op2)) => I_ADD b op1 op2 end
+                          %% i_instr5_t)} :::
+    {22, AND_p false, (fun v => match v with (b,(op1,op2)) => I_AND b op1 op2 end
+                          %% i_instr5_t)} :::
+    {23, BTC_p, (fun v => match v with (op1,op2) => I_BTC op1 op2 end
+                          %% i_instr5_t)} :::
+    {24, BTR_p, (fun v => match v with (op1,op2) => I_BTR op1 op2 end
+                          %% i_instr5_t)} :::
+    {25, BTS_p, (fun v => match v with (op1,op2) => I_BTS op1 op2 end
+                          %% i_instr5_t)} :::
+    {26, CMPXCHG_p, (fun v => match v with (b,(op1,op2)) => I_CMPXCHG b op1 op2 end
+                          %% i_instr5_t)} :::
+    {27, DEC_p, (fun v => match v with (b,op) => I_DEC b op end
+                          %% i_instr5_t)} :::
+    {28, INC_p, (fun v => match v with (b,op) => I_INC b op end
+                          %% i_instr5_t)} :::
+    {29, NEG_p, (fun v => match v with (b,op) => I_NEG b op end
+                          %% i_instr5_t)} :::
+    {30, NOT_p, (fun v => match v with (b,op) => I_NOT b op end
+                          %% i_instr5_t)} :::
+    {31, OR_p false, (fun v => match v with (b,(op1,op2)) => I_OR b op1 op2 end
+                          %% i_instr5_t)} :::
+    {32, SBB_p false, (fun v => match v with (b,(op1,op2)) => I_SBB b op1 op2 end
+                          %% i_instr5_t)} :::
+    {33, SUB_p false, (fun v => match v with (b,(op1,op2)) => I_SUB b op1 op2 end
+                          %% i_instr5_t)} :::
+    {34, XADD_p, (fun v => match v with (b,(op1,op2)) => I_XADD b op1 op2 end
+                          %% i_instr5_t)} :::
+    {35, XCHG_p, (fun v => match v with (b,(op1,op2)) => I_XCHG b op1 op2 end
+                          %% i_instr5_t)} :::
+    {36, XOR_p false, (fun v => match v with (b,(op1,op2)) => I_XOR b op1 op2 end
+                          %% i_instr5_t)} :::
+    ast_env_nil.
+
+  (* this set of instructions can take prefixes in 
+     prefix_grammar_seg_with_op_override;
+     that is, it cannot take a lock_or_rep prefix, must take op_override
+     prefix, can optionally take segment-override prefix *)
+  Definition prefix_seg_with_op_override_env : AST_Env i_instr5_t :=
+    {40, CMP_p true, (fun v => match v with (b,(op1,op2)) => I_CMP b op1 op2 end
+                          %% i_instr5_t)} :::
+    {41, IMUL_p true, (fun v => match v with (b,(op1,(opopt,iopt))) =>
+                                   I_IMUL b op1 opopt iopt end
+                          %% i_instr5_t)} :::
+    {42, MOV_p true, (fun v => match v with (b,(op1,op2)) => I_MOV b op1 op2 end
+                          %% i_instr5_t)} :::
+    {43, TEST_p true, (fun v => match v with (b,(op1,op2)) => I_TEST b op1 op2 end
+                          %% i_instr5_t)} :::
+    ast_env_nil.
+
+
+  (* this set of instructions can take prefixes in 
+     prefix_grammar_seg_with_op_override;
+     that is, it cannot take a lock_or_rep prefix, must take op_override
+     prefix, can optionally take segment-override prefix *)
+  Definition prefix_only_seg_override_env : AST_Env i_instr5_t :=
+    {50, CMP_p false, (fun v => match v with (b,(op1,op2)) => I_CMP b op1 op2 end
+                          %% i_instr5_t)} :::
+    {51, IMUL_p false, (fun v => match v with (b,(op1,(opopt,iopt))) =>
+                                   I_IMUL b op1 opopt iopt end
+                          %% i_instr5_t)} :::
+    {52, MOV_p false, (fun v => match v with (b,(op1,op2)) => I_MOV b op1 op2 end
+                          %% i_instr5_t)} :::
+    {53, TEST_p false, (fun v => match v with (b,(op1,op2)) => I_TEST b op1 op2 end
+                          %% i_instr5_t)} :::
+    ast_env_nil.
+
+
+  Hint Unfold prefix_lock_with_op_override_env prefix_lock_no_op_override_env
+       prefix_seg_with_op_override_env prefix_only_seg_override_env : env_unfold_db.
+
+  Definition i_instr5_grammar_env' := 
+    (ast_env_cat prefix_grammar_lock_with_op_override
+       prefix_lock_with_op_override_env)
+      +++
+    (ast_env_cat prefix_grammar_lock_no_op_override
+       prefix_lock_no_op_override_env)
+      +++
+    (ast_env_cat prefix_grammar_seg_with_op_override
+       prefix_seg_with_op_override_env)
+      +++
+    (ast_env_cat prefix_grammar_only_seg_override
+       prefix_only_seg_override_env).
+
+  Definition i_instr5_grammar_env : AST_Env (pair_t prefix_t i_instr5_t).
+    let ige := eval cbv beta
+                    delta [i_instr5_grammar_env'
+                           prefix_lock_with_op_override_env
+                           prefix_lock_no_op_override_env
+                           prefix_seg_with_op_override_env
+                           prefix_only_seg_override_env
+                           ast_env_app ast_env_cat]
+                    iota zeta 
+               in i_instr5_grammar_env' in
+    exact(ige).
+  Defined.
+
+  Definition i_instr5_grammar_type : type.
+    let ige := eval unfold i_instr5_grammar_env in i_instr5_grammar_env in
+    let t:=gen_ast_type ige in exact(t).
+  Defined.
+
+  Definition from_instr5 (u:prefix * i_instr5) : option [|i_instr5_grammar_type|].
+    intro.
+    refine (match snd u with
+              | I_ADC a1 a2 a3 => _
+              | I_ADD a1 a2 a3 => _
+              | I_AND a1 a2 a3 => _
+              | I_BTC a1 a2 => _
+              | I_BTR a1 a2 => _
+              | I_BTS a1 a2 => _
+              | I_CMP a1 a2 a3 => _
+              | I_CMPXCHG a1 a2 a3 => _
+              | I_DEC a1 a2 => _
+              | I_IMUL a1 a2 a3 a4 => _
+              | I_INC a1 a2 => _
+              | I_MOV a1 a2 a3 => _
+              | I_NEG a1 a2 => _
+              | I_NOT a1 a2 => _
+              | I_OR a1 a2 a3 => _
+              | I_SBB a1 a2 a3 => _
+              | I_SUB a1 a2 a3 => _
+              | I_TEST a1 a2 a3 => _
+              | I_XADD a1 a2 a3 => _
+              | I_XCHG a1 a2 a3 => _
+              | I_XOR a1 a2 a3 => _
+            end).
+    Local Ltac gen5 lbl u arg :=
+      let ige := eval unfold i_instr5_grammar_env
+                 in i_instr5_grammar_env in
+      let t := eval unfold i_instr5_grammar_type
+                 in i_instr5_grammar_type in
+      let f:=gen_rev_case_lbl lbl ige t in
+      let f1 := eval simpl in f in
+      exact (Some (f1 (fst u, arg))).
+    Local Ltac gen_op_override lbl1 lbl2 u arg := 
+      refine (if (op_override (fst u)) then _ else _);
+      [gen5 lbl1 u arg | gen5 lbl2 u arg].
+    * (* ADC *) gen_op_override 0 20 u (a1,(a2,a3)).
+    * (* ADD *)  gen_op_override 1 21 u (a1,(a2,a3)).
+    * (* AND *)  gen_op_override 2 22 u (a1,(a2,a3)).
+    * (* BTC *) gen5 23 u (a1,a2).
+    * (* BTR *) gen5 24 u (a1,a2).
+    * (* BTS *) gen5 25 u (a1,a2).
+    * (* CMP *)  gen_op_override 40 50 u (a1,(a2,a3)).
+    * (* CMPXCHG *) gen5 26 u (a1,(a2,a3)).
+    * (* DEC *) gen5 27 u (a1,a2).
+    * (* IMUL *)  gen_op_override 41 51 u (a1,(a2,(a3,a4))).
+    * (* INC *) gen5 28 u (a1,a2).
+    * (* MOV *)  gen_op_override 42 52 u (a1,(a2,a3)).
+    * (* NEG *) gen_op_override 3 29 u (a1,a2).
+    * (* NOT *) gen_op_override 4 30 u (a1,a2).
+    * (* OR *)  gen_op_override 5 31 u (a1,(a2,a3)).
+    * (* SBB *)  gen_op_override 6 32 u (a1,(a2,a3)).
+    * (* SUB *)  gen_op_override 7 33 u (a1,(a2,a3)).
+    * (* TEST *)  gen_op_override 43 53 u (a1,(a2,a3)).
+    * (* XADD *) gen5 34 u (a1,(a2,a3)).
+    * (* XCHG *) gen_op_override 8 35 u (a1,(a2,a3)).
+    * (* XOR *)  gen_op_override 9 36 u (a1,(a2,a3)).
+  Defined.
+    
+  Definition i_instr5_grammar : wf_bigrammar (pair_t prefix_t i_instr5_t).
+    let ige := eval unfold i_instr5_grammar_env in i_instr5_grammar_env in
+    let g := gen_ast_grammar ige in pose (gr:=g);
+    let m := gen_ast_map ige in pose (mp:=m).
+    Time refine (gr @ (mp: _ -> [|pair_t prefix_t i_instr5_t|])
+                 & from_instr5
+                 & _); clear_ast_defs; unfold from_instr5;
+    unfold invertible; split; [unfold printable | unfold parsable];
+    compute [snd fst]; intros.
+    - abstract instr_printable.
+    - abstract (destruct w as [p ins]; destruct ins; ins_parsable).
+  Defined.
+
+  Definition i_instr6_env : AST_Env i_instr6_t := 
+    {0, CDQ_p, (fun v => I_CDQ %% i_instr6_t)} :::
+    {1, CMOVcc_p, (fun v => match v with (ct,(op1,op2)) => I_CMOVcc ct op1 op2
+                          end %% i_instr6_t)} :::
+    {2, CWDE_p, (fun v => I_CWDE %% i_instr6_t)} :::
+    {3, DIV_p, (fun v => match v with (w,op1) => I_DIV w op1
+                          end %% i_instr6_t)} :::
+    {4, IDIV_p, (fun v => match v with (w,op1) => I_IDIV w op1
+                          end %% i_instr6_t)} :::
+    {5, MOVSX_p, (fun v => match v with (w,(op1,op2)) => I_MOVSX w op1 op2
+                          end %% i_instr6_t)} :::
+    {6, MOVZX_p, (fun v => match v with (w,(op1,op2)) => I_MOVZX w op1 op2
+                          end %% i_instr6_t)} :::
+    {7, MUL_p, (fun v => match v with (w,op1) => I_MUL w op1
+                          end %% i_instr6_t)} :::
+    {8, NOP_p, (fun op => I_NOP op %% i_instr6_t)} :::
+    {9, ROL_p, (fun v => match v with (w,(op1,ri)) => I_ROL w op1 ri
+                          end %% i_instr6_t)} :::
+    {10, ROR_p, (fun v => match v with (w,(op1,ri)) => I_ROR w op1 ri
+                          end %% i_instr6_t)} :::
+    {11, SAR_p, (fun v => match v with (w,(op1,ri)) => I_SAR w op1 ri
+                          end %% i_instr6_t)} :::
+    {12, SHL_p, (fun v => match v with (w,(op1,ri)) => I_SHL w op1 ri
+                          end %% i_instr6_t)} :::
+    {13, SHLD_p, (fun v => match v with (op1,(r,ri)) => I_SHLD op1 r ri
+                          end %% i_instr6_t)} :::
+    {14, SHR_p, (fun v => match v with (w,(op1,ri)) => I_SHR w op1 ri
+                          end %% i_instr6_t)} :::
+    {15, SHRD_p, (fun v => match v with (op1,(r,ri)) => I_SHRD op1 r ri
+                          end %% i_instr6_t)} :::
+    ast_env_nil.
+  Hint Unfold i_instr6_env: env_unfold_db.
+
+  Definition i_instr6_p : wf_bigrammar i_instr6_t.
+    gen_ast_defs i_instr6_env.
+    refine (gr @ (mp: _ -> [|i_instr6_t|])
+               & (fun u =>
+                    match u with
+                      | I_CDQ => case0 tt
+                      | I_CMOVcc ct op1 op2 => case1 (ct,(op1,op2))
+                      | I_CWDE => case2 tt
+                      | I_DIV w op1 => case3 (w,op1)
+                      | I_IDIV w op1 => case4 (w,op1)
+                      | I_MOVSX w op1 op2 => case5 (w,(op1,op2))
+                      | I_MOVZX w op1 op2 => case6 (w,(op1,op2))
+                      | I_MUL w op1 => case7 (w,op1)
+                      | I_NOP op => case8 op
+                      | I_ROL w op1 ri => case9 (w,(op1,ri))
+                      | I_ROR w op1 ri => case10 (w,(op1,ri))
+                      | I_SAR w op1 ri => case11 (w,(op1,ri))
+                      | I_SHL w op1 ri => case12 (w,(op1,ri))
+                      | I_SHLD op1 r ri => case13 (op1,(r,ri))
+                      | I_SHR w op1 ri => case14 (w,(op1,ri))
+                      | I_SHRD op1 r ri => case15 (op1,(r,ri))
+                    end)
+               & _); clear_ast_defs;
+    unfold invertible; split; [unfold printable | unfold parsable]; 
+    compute [snd fst]; intros.
+    - repeat match goal with
+               | [v: [| Sum_t _ _ |] |- _ ] => case v as [v | v]
+               | [v: [| unit_t |] |- _] => destruct v
+               | [v:[|pair_t _ _|] |- _] => destruct v
+             end; abstract printable_tac.
+    - abstract (destruct w; parsable_tac).
+  Defined.
+
+  Definition f_instr1_env : AST_Env f_instr1_t := 
+    {0, F2XM1_p, (fun v => F_F2XM1 %% f_instr1_t)} :::
+    {1, FABS_p, (fun v => F_FABS %% f_instr1_t)} :::
+    {2, FADD_p, (fun v => match v with (z,op1) => F_FADD z op1
+                          end %% f_instr1_t)} :::
+    {3, FADDP_p, (fun op => F_FADDP op %% f_instr1_t)} :::
+    {4, FBLD_p, (fun op => F_FBLD op %% f_instr1_t)} :::
+    {5, FBSTP_p, (fun op => F_FBSTP op %% f_instr1_t)} :::
+    {6, FCHS_p, (fun v => F_FCHS %% f_instr1_t)} :::
+    {7, FCMOVcc_p, (fun v => match v with (ct,op1) => F_FCMOVcc ct op1
+                          end %% f_instr1_t)} :::
+    {8, FCOM_p, (fun op => F_FCOM op %% f_instr1_t)} :::
+    {9, FCOMP_p, (fun op => F_FCOMP op %% f_instr1_t)} :::
+    {10, FCOMPP_p, (fun v => F_FCOMPP %% f_instr1_t)} :::
+    {11, FCOMIP_p, (fun op => F_FCOMIP op %% f_instr1_t)} :::
+    {12, FCOS_p, (fun v => F_FCOS %% f_instr1_t)} :::
+    {13, FDECSTP_p, (fun v => F_FDECSTP %% f_instr1_t)} :::
+    {14, FDIV_p, (fun v => match v with (z,op1) => F_FDIV z op1
+                          end %% f_instr1_t)} :::
+    {15, FDIVP_p, (fun op => F_FDIVP op %% f_instr1_t)} :::
+    {16, FDIVR_p, (fun v => match v with (z,op1) => F_FDIVR z op1
+                          end %% f_instr1_t)} :::
+    {17, FDIVRP_p, (fun op => F_FDIVRP op %% f_instr1_t)} :::
+    {18, FFREE_p, (fun op => F_FFREE op %% f_instr1_t)} :::
+    {19, FIADD_p, (fun op => F_FIADD op %% f_instr1_t)} :::
+    {20, FICOM_p, (fun op => F_FICOM op %% f_instr1_t)} :::
+    {21, FICOMP_p, (fun op => F_FICOMP op %% f_instr1_t)} :::
+    {22, FIDIV_p, (fun op => F_FIDIV op %% f_instr1_t)} :::
+    {23, FIDIVR_p, (fun op => F_FIDIVR op %% f_instr1_t)} :::
+    {24, FILD_p, (fun op => F_FILD op %% f_instr1_t)} :::
+    {25, FIMUL_p, (fun op => F_FIMUL op %% f_instr1_t)} :::
+    {26, FINCSTP_p, (fun v => F_FINCSTP %% f_instr1_t)} :::
+    {27, FIST_p, (fun op => F_FIST op %% f_instr1_t)} :::
+    {28, FISTP_p, (fun op => F_FISTP op %% f_instr1_t)} :::
+    {29, FISUB_p, (fun op => F_FISUB op %% f_instr1_t)} :::
+    {30, FISUBR_p, (fun op => F_FISUBR op %% f_instr1_t)} :::
+    {31, FLD_p, (fun op => F_FLD op %% f_instr1_t)} :::
+    {32, FLD1_p, (fun v => F_FLD1 %% f_instr1_t)} :::
+    {33, FLDCW_p, (fun op => F_FLDCW op %% f_instr1_t)} :::
+    {34, FLDENV_p, (fun op => F_FLDENV op %% f_instr1_t)} :::
+    {35, FLDL2E_p, (fun v => F_FLDL2E %% f_instr1_t)} :::
+    {36, FLDL2T_p, (fun v => F_FLDL2T %% f_instr1_t)} :::
+    {37, FLDLG2_p, (fun v => F_FLDLG2 %% f_instr1_t)} :::
+    {38, FLDLN2_p, (fun v => F_FLDLN2 %% f_instr1_t)} :::
+    {39, FLDPI_p, (fun v => F_FLDPI %% f_instr1_t)} :::
+    {40, FLDZ_p, (fun v => F_FLDZ %% f_instr1_t)} :::
+    {41, FMUL_p, (fun v => match v with (z,op1) => F_FMUL z op1
+                          end %% f_instr1_t)} :::
+    {42, FMULP_p, (fun op => F_FMULP op %% f_instr1_t)} :::
+    ast_env_nil.
+  Hint Unfold f_instr1_env: env_unfold_db.
+
+  Definition f_instr1_p : wf_bigrammar f_instr1_t.
+    gen_ast_defs f_instr1_env.
+    refine (gr @ (mp: _ -> [|f_instr1_t|])
+               & (fun u =>
+                    match u with
+                      | F_F2XM1 => case0 tt
+                      | F_FABS => case1 tt
+                      | F_FADD z op1 => case2 (z,op1)
+                      | F_FADDP op => case3 op
+                      | F_FBLD op => case4 op
+                      | F_FBSTP op => case5 op
+                      | F_FCHS => case6 tt
+                      | F_FCMOVcc ct op => case7 (ct,op)
+                      | F_FCOM op => case8 op
+                      | F_FCOMP op => case9 op
+                      | F_FCOMPP => case10 tt
+                      | F_FCOMIP op => case11 op
+                      | F_FCOS => case12 tt
+                      | F_FDECSTP => case13 tt
+                      | F_FDIV z op => case14 (z,op)
+                      | F_FDIVP op => case15 op
+                      | F_FDIVR z op => case16 (z,op)
+                      | F_FDIVRP op => case17 op
+                      | F_FFREE op => case18 op
+                      | F_FIADD op => case19 op
+                      | F_FICOM op => case20 op
+                      | F_FICOMP op => case21 op
+                      | F_FIDIV op => case22 op
+                      | F_FIDIVR op => case23 op
+                      | F_FILD op => case24 op
+                      | F_FIMUL op => case25 op
+                      | F_FINCSTP => case26 tt
+                      | F_FIST op => case27 op
+                      | F_FISTP op => case28 op
+                      | F_FISUB op => case29 op
+                      | F_FISUBR op => case30 op
+                      | F_FLD op => case31 op
+                      | F_FLD1 => case32 tt
+                      | F_FLDCW op => case33 op
+                      | F_FLDENV op => case34 op
+                      | F_FLDL2E => case35 tt
+                      | F_FLDL2T => case36 tt
+                      | F_FLDLG2 => case37 tt
+                      | F_FLDLN2 => case38 tt
+                      | F_FLDPI => case39 tt
+                      | F_FLDZ => case40 tt
+                      | F_FMUL z op => case41 (z,op)
+                      | F_FMULP op => case42 op
+                    end)
+               & _); clear_ast_defs;
+    unfold invertible; split; [unfold printable | unfold parsable]; 
+    compute [snd fst]; intros.
+    - repeat match goal with
+               | [v: [| Sum_t _ _ |] |- _ ] => case v as [v | v]
+               | [v: [| unit_t |] |- _] => destruct v
+               | [v:[|pair_t _ _|] |- _] => destruct v
+             end; abstract printable_tac.
+    - abstract (destruct w; parsable_tac).
+  Defined.
+
+  Definition f_instr2_env : AST_Env f_instr2_t := 
+    {0, FNCLEX_p, (fun v => F_FNCLEX %% f_instr2_t)} :::
+    {1, FNINIT_p, (fun v => F_FNINIT %% f_instr2_t)} :::
+    {2, FNOP_p, (fun v => F_FNOP %% f_instr2_t)} :::
+    {3, FNSAVE_p, (fun op => F_FNSAVE op %% f_instr2_t)} :::
+    {4, FNSTCW_p, (fun op => F_FNSTCW op %% f_instr2_t)} :::
+    {5, FNSTSW_p, (fun op => F_FNSTSW op %% f_instr2_t)} :::
+    {6, FPATAN_p, (fun v => F_FPATAN %% f_instr2_t)} :::
+    {7, FPREM_p, (fun v => F_FPREM %% f_instr2_t)} :::
+    {8, FPREM1_p, (fun v => F_FPREM1 %% f_instr2_t)} :::
+    {9, FPTAN_p, (fun v => F_FPTAN %% f_instr2_t)} :::
+    {10, FRNDINT_p, (fun v => F_FRNDINT %% f_instr2_t)} :::
+    {11, FRSTOR_p, (fun op => F_FRSTOR op %% f_instr2_t)} :::
+    {12, FSCALE_p, (fun v => F_FSCALE %% f_instr2_t)} :::
+    {13, FSIN_p, (fun v => F_FSIN %% f_instr2_t)} :::
+    {14, FSINCOS_p, (fun v => F_FSINCOS %% f_instr2_t)} :::
+    {15, FSQRT_p, (fun v => F_FSQRT %% f_instr2_t)} :::
+    {16, FST_p, (fun op => F_FST op %% f_instr2_t)} :::
+    {17, FSTENV_p, (fun op => F_FSTENV op %% f_instr2_t)} :::
+    {18, FSTP_p, (fun op => F_FSTP op %% f_instr2_t)} :::
+    {19, FSUB_p, (fun v => match v with (z,op) => F_FSUB z op 
+                           end %% f_instr2_t)} :::
+    {20, FSUBP_p, (fun op => F_FSUBP op %% f_instr2_t)} :::
+    {21, FSUBR_p, (fun v => match v with (z,op) => F_FSUBR z op 
+                           end %% f_instr2_t)} :::
+    {22, FSUBRP_p, (fun op => F_FSUBRP op %% f_instr2_t)} :::
+    {23, FTST_p, (fun v => F_FTST %% f_instr2_t)} :::
+    {24, FUCOM_p, (fun op => F_FUCOM op %% f_instr2_t)} :::
+    {25, FUCOMP_p, (fun op => F_FUCOMP op %% f_instr2_t)} :::
+    {26, FUCOMPP_p, (fun v => F_FUCOMPP %% f_instr2_t)} :::
+    {27, FUCOMI_p, (fun op => F_FUCOMI op %% f_instr2_t)} :::
+    {28, FUCOMIP_p, (fun op => F_FUCOMIP op %% f_instr2_t)} :::
+    {29, FXAM_p, (fun v => F_FXAM %% f_instr2_t)} :::
+    {30, FXCH_p, (fun op => F_FXCH op %% f_instr2_t)} :::
+    {31, FXTRACT_p, (fun v => F_FXTRACT %% f_instr2_t)} :::
+    {32, FYL2X_p, (fun v => F_FYL2X %% f_instr2_t)} :::
+    {33, FYL2XP1_p, (fun v => F_FYL2XP1 %% f_instr2_t)} :::
+    {34, FWAIT_p, (fun v => F_FWAIT %% f_instr2_t)} :::
+    ast_env_nil.
+  Hint Unfold f_instr2_env: env_unfold_db.
+
+  Definition f_instr2_p : wf_bigrammar f_instr2_t.
+    gen_ast_defs f_instr2_env.
+    refine (gr @ (mp: _ -> [|f_instr2_t|])
+               & (fun u =>
+                    match u with
+                      | F_FNCLEX => case0 tt
+                      | F_FNINIT => case1 tt
+                      | F_FNOP => case2 tt
+                      | F_FNSAVE op => case3 op
+                      | F_FNSTCW op => case4 op
+                      | F_FNSTSW op => case5 op
+                      | F_FPATAN => case6 tt
+                      | F_FPREM => case7 tt
+                      | F_FPREM1 => case8 tt
+                      | F_FPTAN => case9 tt
+                      | F_FRNDINT => case10 tt
+                      | F_FRSTOR op => case11 op
+                      | F_FSCALE => case12 tt
+                      | F_FSIN => case13 tt
+                      | F_FSINCOS => case14 tt
+                      | F_FSQRT => case15 tt
+                      | F_FST op => case16 op
+                      | F_FSTENV op => case17 op
+                      | F_FSTP op => case18 op
+                      | F_FSUB z op => case19 (z,op)
+                      | F_FSUBP op => case20 op
+                      | F_FSUBR z op => case21 (z,op)
+                      | F_FSUBRP op => case22 op
+                      | F_FTST => case23 tt
+                      | F_FUCOM op => case24 op
+                      | F_FUCOMP op => case25 op
+                      | F_FUCOMPP => case26 tt
+                      | F_FUCOMI op => case27 op
+                      | F_FUCOMIP op => case28 op
+                      | F_FXAM => case29 tt
+                      | F_FXCH op => case30 op
+                      | F_FXTRACT => case31 tt
+                      | F_FYL2X => case32 tt
+                      | F_FYL2XP1 => case33 tt
+                      | F_FWAIT => case34 tt
+                    end)
+               & _); clear_ast_defs;
+    unfold invertible; split; [unfold printable | unfold parsable]; 
+    compute [snd fst]; intros.
+    - repeat match goal with
+               | [v: [| Sum_t _ _ |] |- _ ] => case v as [v | v]
+               | [v: [| unit_t |] |- _] => destruct v
+               | [v:[|pair_t _ _|] |- _] => destruct v
+             end; abstract printable_tac.
+    - abstract (destruct w; parsable_tac).
+  Defined.
+
+  Definition m_instr_env : AST_Env m_instr_t := 
+    {0, EMMS_p, (fun v => M_EMMS %% m_instr_t)} :::
+    {1, MOVD_p, (fun v => match v with (op1,op2) => M_MOVD op1 op2
+                          end %% m_instr_t)} :::
+    {2, MOVQ_p, (fun v => match v with (op1,op2) => M_MOVQ op1 op2
+                          end %% m_instr_t)} :::
+    {3, PACKSSDW_p, (fun v => match v with (op1,op2) => M_PACKSSDW op1 op2
+                          end %% m_instr_t)} :::
+    {4, PACKSSWB_p, (fun v => match v with (op1,op2) => M_PACKSSWB op1 op2
+                          end %% m_instr_t)} :::
+    {5, PACKUSWB_p, (fun v => match v with (op1,op2) => M_PACKUSWB op1 op2
+                          end %% m_instr_t)} :::
+    {6, PADD_p, (fun v => match v with (gg,(op1,op2)) => M_PADD gg op1 op2
+                          end %% m_instr_t)} :::
+    {7, PADDS_p, (fun v => match v with (gg,(op1,op2)) => M_PADDS gg op1 op2
+                          end %% m_instr_t)} :::
+    {8, PADDUS_p, (fun v => match v with (gg,(op1,op2)) => M_PADDUS gg op1 op2
+                          end %% m_instr_t)} :::
+    {9, PAND_p, (fun v => match v with (op1,op2) => M_PAND op1 op2
+                          end %% m_instr_t)} :::
+    {10, PANDN_p, (fun v => match v with (op1,op2) => M_PANDN op1 op2
+                          end %% m_instr_t)} :::
+    {11, PCMPEQ_p, (fun v => match v with (gg,(op1,op2)) => M_PCMPEQ gg op1 op2
+                          end %% m_instr_t)} :::
+    {12, PCMPGT_p, (fun v => match v with (gg,(op1,op2)) => M_PCMPGT gg op1 op2
+                          end %% m_instr_t)} :::
+    {13, PMADDWD_p, (fun v => match v with (op1,op2) => M_PMADDWD op1 op2
+                          end %% m_instr_t)} :::
+    {14, PMULHUW_p, (fun v => match v with (op1,op2) => M_PMULHUW op1 op2
+                          end %% m_instr_t)} :::
+    {15, PMULHW_p, (fun v => match v with (op1,op2) => M_PMULHW op1 op2
+                          end %% m_instr_t)} :::
+    {16, PMULLW_p, (fun v => match v with (op1,op2) => M_PMULLW op1 op2
+                          end %% m_instr_t)} :::
+    {17, POR_p, (fun v => match v with (op1,op2) => M_POR op1 op2
+                          end %% m_instr_t)} :::
+    {18, PSLL_p, (fun v => match v with (gg,(op1,op2)) => M_PSLL gg op1 op2
+                          end %% m_instr_t)} :::
+    {19, PSRA_p, (fun v => match v with (gg,(op1,op2)) => M_PSRA gg op1 op2
+                          end %% m_instr_t)} :::
+    {20, PSRL_p, (fun v => match v with (gg,(op1,op2)) => M_PSRL gg op1 op2
+                          end %% m_instr_t)} :::
+    {20, PSUB_p, (fun v => match v with (gg,(op1,op2)) => M_PSUB gg op1 op2
+                          end %% m_instr_t)} :::
+    {22, PSUBS_p, (fun v => match v with (gg,(op1,op2)) => M_PSUBS gg op1 op2
+                          end %% m_instr_t)} :::
+    {23, PSUBUS_p, (fun v => match v with (gg,(op1,op2)) => M_PSUBUS gg op1 op2
+                          end %% m_instr_t)} :::
+    {24, PUNPCKH_p, (fun v => match v with (gg,(op1,op2)) => M_PUNPCKH gg op1 op2
+                          end %% m_instr_t)} :::
+    {25, PUNPCKL_p, (fun v => match v with (gg,(op1,op2)) => M_PUNPCKL gg op1 op2
+                          end %% m_instr_t)} :::
+    {26, PXOR_p, (fun v => match v with (op1,op2) => M_PXOR op1 op2
+                          end %% m_instr_t)} :::
+    ast_env_nil.
+  Hint Unfold m_instr_env: env_unfold_db.
+
+  Definition m_instr_p : wf_bigrammar m_instr_t.
+    gen_ast_defs m_instr_env.
+    refine (gr @ (mp: _ -> [|m_instr_t|])
+               & (fun u =>
+                    match u with
+                      | M_EMMS => case0 tt
+                      | M_MOVD op1 op2 => case1 (op1,op2)
+                      | M_MOVQ op1 op2 => case2 (op1,op2)
+                      | M_PACKSSDW op1 op2 => case3 (op1,op2)
+                      | M_PACKSSWB op1 op2 => case4 (op1,op2)
+                      | M_PACKUSWB op1 op2 => case5 (op1,op2)
+                      | M_PADD gg op1 op2 => case6 (gg,(op1,op2))
+                      | M_PADDS gg op1 op2 => case7 (gg,(op1,op2))
+                      | M_PADDUS gg op1 op2 => case8 (gg,(op1,op2))
+                      | M_PAND op1 op2 => case9 (op1,op2)
+                      | M_PANDN op1 op2 => case10 (op1,op2)
+                      | M_PCMPEQ gg op1 op2 => case11 (gg,(op1,op2))
+                      | M_PCMPGT gg op1 op2 => case12 (gg,(op1,op2))
+                      | M_PMADDWD op1 op2 => case13 (op1,op2)
+                      | M_PMULHUW op1 op2 => case14 (op1,op2)
+                      | M_PMULHW op1 op2 => case15 (op1,op2)
+                      | M_PMULLW op1 op2 => case16 (op1,op2)
+                      | M_POR op1 op2 => case17 (op1,op2)
+                      | M_PSLL gg op1 op2 => case18 (gg,(op1,op2))
+                      | M_PSRA gg op1 op2 => case19 (gg,(op1,op2))
+                      | M_PSRL gg op1 op2 => case20 (gg,(op1,op2))
+                      | M_PSUB gg op1 op2 => case21 (gg,(op1,op2))
+                      | M_PSUBS gg op1 op2 => case22 (gg,(op1,op2))
+                      | M_PSUBUS gg op1 op2 => case23 (gg,(op1,op2))
+                      | M_PUNPCKH gg op1 op2 => case24 (gg,(op1,op2))
+                      | M_PUNPCKL gg op1 op2 => case25 (gg,(op1,op2))
+                      | M_PXOR op1 op2 => case26 (op1,op2)
+                    end)
+               & _); clear_ast_defs;
+    unfold invertible; split; [unfold printable | unfold parsable]; 
+    compute [snd fst]; intros.
+    - repeat match goal with
+               | [v: [| Sum_t _ _ |] |- _ ] => case v as [v | v]
+               | [v: [| unit_t |] |- _] => destruct v
+               | [v:[|pair_t _ _|] |- _] => destruct v
+             end; abstract printable_tac.
+    - abstract (destruct w; parsable_tac).
+  Defined.
+
+  Definition s_instr1_env : AST_Env s_instr1_t := 
+    {0, ADDPS_p, (fun v => match v with (op1,op2) => S_ADDPS op1 op2
+                          end %% s_instr1_t)} :::
+    {1, ADDSS_p, (fun v => match v with (op1,op2) => S_ADDSS op1 op2
+                          end %% s_instr1_t)} :::
+    {2, ANDNPS_p, (fun v => match v with (op1,op2) => S_ANDNPS op1 op2
+                          end %% s_instr1_t)} :::
+    {3, ANDPS_p, (fun v => match v with (op1,op2) => S_ANDPS op1 op2
+                          end %% s_instr1_t)} :::
+    {4, CMPPS_p, (fun v => match v with (op1,(op2,imm)) => S_CMPPS op1 op2 imm
+                          end %% s_instr1_t)} :::
+    {5, CMPSS_p, (fun v => match v with (op1,(op2,imm)) => S_CMPSS op1 op2 imm
+                          end %% s_instr1_t)} :::
+    {6, COMISS_p, (fun v => match v with (op1,op2) => S_COMISS op1 op2
+                          end %% s_instr1_t)} :::
+    {7, CVTPI2PS_p, (fun v => match v with (op1,op2) => S_CVTPI2PS op1 op2
+                          end %% s_instr1_t)} :::
+    {8, CVTPS2PI_p, (fun v => match v with (op1,op2) => S_CVTPS2PI op1 op2
+                          end %% s_instr1_t)} :::
+    {9, CVTSI2SS_p, (fun v => match v with (op1,op2) => S_CVTSI2SS op1 op2
+                          end %% s_instr1_t)} :::
+    {10, CVTSS2SI_p, (fun v => match v with (op1,op2) => S_CVTSS2SI op1 op2
+                          end %% s_instr1_t)} :::
+    {11, CVTTPS2PI_p, (fun v => match v with (op1,op2) => S_CVTTPS2PI op1 op2
+                          end %% s_instr1_t)} :::
+    {12, CVTTSS2SI_p, (fun v => match v with (op1,op2) => S_CVTTSS2SI op1 op2
+                          end %% s_instr1_t)} :::
+    {13, DIVPS_p, (fun v => match v with (op1,op2) => S_DIVPS op1 op2
+                          end %% s_instr1_t)} :::
+    {14, DIVSS_p, (fun v => match v with (op1,op2) => S_DIVSS op1 op2
+                          end %% s_instr1_t)} :::
+    {15, LDMXCSR_p, (fun op => S_LDMXCSR op %% s_instr1_t)} :::
+    {16, MAXPS_p, (fun v => match v with (op1,op2) => S_MAXPS op1 op2
+                          end %% s_instr1_t)} :::
+    {17, MAXSS_p, (fun v => match v with (op1,op2) => S_MAXSS op1 op2
+                          end %% s_instr1_t)} :::
+    {18, MINPS_p, (fun v => match v with (op1,op2) => S_MINPS op1 op2
+                          end %% s_instr1_t)} :::
+    {19, MINSS_p, (fun v => match v with (op1,op2) => S_MINSS op1 op2
+                          end %% s_instr1_t)} :::
+    {20, MOVAPS_p, (fun v => match v with (op1,op2) => S_MOVAPS op1 op2
+                          end %% s_instr1_t)} :::
+    {21, MOVHLPS_p, (fun v => match v with (op1,op2) => S_MOVHLPS op1 op2
+                          end %% s_instr1_t)} :::
+    {22, MOVHPS_p, (fun v => match v with (op1,op2) => S_MOVHPS op1 op2
+                          end %% s_instr1_t)} :::
+    {23, MOVLHPS_p, (fun v => match v with (op1,op2) => S_MOVLHPS op1 op2
+                          end %% s_instr1_t)} :::
+    {24, MOVLPS_p, (fun v => match v with (op1,op2) => S_MOVLPS op1 op2
+                          end %% s_instr1_t)} :::
+    {25, MOVMSKPS_p, (fun v => match v with (op1,op2) => S_MOVMSKPS op1 op2
+                          end %% s_instr1_t)} :::
+    {26, MOVSS_p, (fun v => match v with (op1,op2) => S_MOVSS op1 op2
+                          end %% s_instr1_t)} :::
+    {27, MOVUPS_p, (fun v => match v with (op1,op2) => S_MOVUPS op1 op2
+                          end %% s_instr1_t)} :::
+    {28, MULPS_p, (fun v => match v with (op1,op2) => S_MULPS op1 op2
+                          end %% s_instr1_t)} :::
+    {29, MULSS_p, (fun v => match v with (op1,op2) => S_MULSS op1 op2
+                          end %% s_instr1_t)} :::
+    {30, ORPS_p, (fun v => match v with (op1,op2) => S_ORPS op1 op2
+                          end %% s_instr1_t)} :::
+    {31, RCPPS_p, (fun v => match v with (op1,op2) => S_RCPPS op1 op2
+                          end %% s_instr1_t)} :::
+    {32, RCPSS_p, (fun v => match v with (op1,op2) => S_RCPSS op1 op2
+                          end %% s_instr1_t)} :::
+    {33, RSQRTPS_p, (fun v => match v with (op1,op2) => S_RSQRTPS op1 op2
+                          end %% s_instr1_t)} :::
+    {34, RSQRTSS_p, (fun v => match v with (op1,op2) => S_RSQRTSS op1 op2
+                          end %% s_instr1_t)} :::
+    ast_env_nil.
+  Hint Unfold s_instr1_env: env_unfold_db.
+
+  Definition s_instr1_p : wf_bigrammar s_instr1_t.
+    gen_ast_defs s_instr1_env.
+    refine (gr @ (mp: _ -> [|s_instr1_t|])
+               & (fun u =>
+                    match u with
+                      | S_ADDPS op1 op2 => case0 (op1,op2)
+                      | S_ADDSS op1 op2 => case1 (op1,op2)
+                      | S_ANDNPS op1 op2 => case2 (op1,op2)
+                      | S_ANDPS op1 op2 => case3 (op1,op2)
+                      | S_CMPPS op1 op2 imm => case4 (op1,(op2,imm))
+                      | S_CMPSS op1 op2 imm => case5 (op1,(op2,imm))
+                      | S_COMISS op1 op2 => case6 (op1,op2)
+                      | S_CVTPI2PS op1 op2 => case7 (op1,op2)
+                      | S_CVTPS2PI op1 op2 => case8 (op1,op2)
+                      | S_CVTSI2SS op1 op2 => case9 (op1,op2)
+                      | S_CVTSS2SI op1 op2 => case10 (op1,op2)
+                      | S_CVTTPS2PI op1 op2 => case11 (op1,op2)
+                      | S_CVTTSS2SI op1 op2 => case12 (op1,op2)
+                      | S_DIVPS op1 op2 => case13 (op1,op2)
+                      | S_DIVSS op1 op2 => case14 (op1,op2)
+                      | S_LDMXCSR op => case15 op
+                      | S_MAXPS op1 op2 => case16 (op1,op2)
+                      | S_MAXSS op1 op2 => case17 (op1,op2)
+                      | S_MINPS op1 op2 => case18 (op1,op2)
+                      | S_MINSS op1 op2 => case19 (op1,op2)
+                      | S_MOVAPS op1 op2 => case20 (op1,op2)
+                      | S_MOVHLPS op1 op2 => case21 (op1,op2)
+                      | S_MOVHPS op1 op2 => case22 (op1,op2)
+                      | S_MOVLHPS op1 op2 => case23 (op1,op2)
+                      | S_MOVLPS op1 op2 => case24 (op1,op2)
+                      | S_MOVMSKPS op1 op2 => case25 (op1,op2)
+                      | S_MOVSS op1 op2 => case26 (op1,op2)
+                      | S_MOVUPS op1 op2 => case27 (op1,op2)
+                      | S_MULPS op1 op2 => case28 (op1,op2)
+                      | S_MULSS op1 op2 => case29 (op1,op2)
+                      | S_ORPS op1 op2 => case30 (op1,op2)
+                      | S_RCPPS op1 op2 => case31 (op1,op2)
+                      | S_RCPSS op1 op2 => case32 (op1,op2)
+                      | S_RSQRTPS op1 op2 => case33 (op1,op2)
+                      | S_RSQRTSS op1 op2 => case34 (op1,op2)
+                    end)
+               & _); clear_ast_defs;
+    unfold invertible; split; [unfold printable | unfold parsable]; 
+    compute [snd fst]; intros.
+    - repeat match goal with
+               | [v: [| Sum_t _ _ |] |- _ ] => case v as [v | v]
+               | [v: [| unit_t |] |- _] => destruct v
+               | [v:[|pair_t _ _|] |- _] => destruct v
+             end; abstract printable_tac.
+    - abstract (destruct w; parsable_tac).
+  Defined.
+
+  Definition s_instr2_env : AST_Env s_instr2_t := 
+    {0, SHUFPS_p, (fun v => match v with (op1,(op2,imm)) => S_SHUFPS op1 op2 imm
+                          end %% s_instr2_t)} :::
+    {1, SQRTPS_p, (fun v => match v with (op1,op2) => S_SQRTPS op1 op2
+                          end %% s_instr2_t)} :::
+    {2, SQRTSS_p, (fun v => match v with (op1,op2) => S_SQRTSS op1 op2
+                          end %% s_instr2_t)} :::
+    {3, STMXCSR_p, (fun op => S_STMXCSR op %% s_instr2_t)} :::
+    {4, SUBPS_p, (fun v => match v with (op1,op2) => S_SUBPS op1 op2
+                          end %% s_instr2_t)} :::
+    {5, SUBSS_p, (fun v => match v with (op1,op2) => S_SUBSS op1 op2
+                          end %% s_instr2_t)} :::
+    {6, UCOMISS_p, (fun v => match v with (op1,op2) => S_UCOMISS op1 op2
+                          end %% s_instr2_t)} :::
+    {7, UNPCKHPS_p, (fun v => match v with (op1,op2) => S_UNPCKHPS op1 op2
+                          end %% s_instr2_t)} :::
+    {8, UNPCKLPS_p, (fun v => match v with (op1,op2) => S_UNPCKLPS op1 op2
+                          end %% s_instr2_t)} :::
+    {9, XORPS_p, (fun v => match v with (op1,op2) => S_XORPS op1 op2
+                          end %% s_instr2_t)} :::
+    {10, PAVGB_p, (fun v => match v with (op1,op2) => S_PAVGB op1 op2
+                          end %% s_instr2_t)} :::
+    {11, PEXTRW_p, (fun v => match v with (op1,(op2,imm)) => S_PEXTRW op1 op2 imm
+                          end %% s_instr2_t)} :::
+    {12, PINSRW_p, (fun v => match v with (op1,(op2,imm)) => S_PINSRW op1 op2 imm
+                          end %% s_instr2_t)} :::
+    {13, PMAXSW_p, (fun v => match v with (op1,op2) => S_PMAXSW op1 op2
+                          end %% s_instr2_t)} :::
+    {14, PMAXUB_p, (fun v => match v with (op1,op2) => S_PMAXUB op1 op2
+                          end %% s_instr2_t)} :::
+    {15, PMINSW_p, (fun v => match v with (op1,op2) => S_PMINSW op1 op2
+                          end %% s_instr2_t)} :::
+    {16, PMINUB_p, (fun v => match v with (op1,op2) => S_PMINUB op1 op2
+                          end %% s_instr2_t)} :::
+    {17, PMOVMSKB_p, (fun v => match v with (op1,op2) => S_PMOVMSKB op1 op2
+                          end %% s_instr2_t)} :::
+    {18, PSADBW_p, (fun v => match v with (op1,op2) => S_PSADBW op1 op2
+                          end %% s_instr2_t)} :::
+    {19, PSHUFW_p, (fun v => match v with (op1,(op2,imm)) => S_PSHUFW op1 op2 imm
+                          end %% s_instr2_t)} :::
+    {20, MASKMOVQ_p, (fun v => match v with (op1,op2) => S_MASKMOVQ op1 op2
+                          end %% s_instr2_t)} :::
+    {21, MOVNTPS_p, (fun v => match v with (op1,op2) => S_MOVNTPS op1 op2
+                          end %% s_instr2_t)} :::
+    {22, MOVNTQ_p, (fun v => match v with (op1,op2) => S_MOVNTQ op1 op2
+                          end %% s_instr2_t)} :::
+    {23, PREFETCHT0_p, (fun op => S_PREFETCHT0 op %% s_instr2_t)} :::
+    {24, PREFETCHT1_p, (fun op => S_PREFETCHT1 op %% s_instr2_t)} :::
+    {25, PREFETCHT2_p, (fun op => S_PREFETCHT2 op %% s_instr2_t)} :::
+    {26, PREFETCHNTA_p, (fun op => S_PREFETCHNTA op %% s_instr2_t)} :::
+    {27, SFENCE_p, (fun v => S_SFENCE %% s_instr2_t)} :::
+    ast_env_nil.
+  Hint Unfold s_instr2_env: env_unfold_db.
+
+  Definition s_instr2_p : wf_bigrammar s_instr2_t.
+    gen_ast_defs s_instr2_env.
+    refine (gr @ (mp: _ -> [|s_instr2_t|])
+               & (fun u =>
+                    match u with
+                      | S_SHUFPS op1 op2 imm => case0 (op1,(op2,imm))
+                      | S_SQRTPS op1 op2 => case1 (op1,op2)
+                      | S_SQRTSS op1 op2 => case2 (op1,op2)
+                      | S_STMXCSR op => case3 op
+                      | S_SUBPS op1 op2 => case4 (op1,op2)
+                      | S_SUBSS op1 op2 => case5 (op1,op2)
+                      | S_UCOMISS op1 op2 => case6 (op1,op2)
+                      | S_UNPCKHPS op1 op2 => case7 (op1,op2)
+                      | S_UNPCKLPS op1 op2 => case8 (op1,op2)
+                      | S_XORPS op1 op2 => case9 (op1,op2)
+                      | S_PAVGB op1 op2 => case10 (op1,op2)
+                      | S_PEXTRW op1 op2 imm => case11 (op1,(op2,imm))
+                      | S_PINSRW op1 op2 imm => case12 (op1,(op2,imm))
+                      | S_PMAXSW op1 op2 => case13 (op1,op2)
+                      | S_PMAXUB op1 op2 => case14 (op1,op2)
+                      | S_PMINSW op1 op2 => case15 (op1,op2)
+                      | S_PMINUB op1 op2 => case16 (op1,op2)
+                      | S_PMOVMSKB op1 op2 => case17 (op1,op2)
+                      | S_PSADBW op1 op2 => case18 (op1,op2)
+                      | S_PSHUFW op1 op2 imm => case19 (op1,(op2,imm))
+                      | S_MASKMOVQ op1 op2 => case20 (op1,op2)
+                      | S_MOVNTPS op1 op2 => case21 (op1,op2)
+                      | S_MOVNTQ op1 op2 => case22 (op1,op2)
+                      | S_PREFETCHT0 op => case23 op
+                      | S_PREFETCHT1 op => case24 op
+                      | S_PREFETCHT2 op => case25 op
+                      | S_PREFETCHNTA op => case26 op
+                      | S_SFENCE => case27 tt
+                    end)
+               & _); clear_ast_defs;
+    unfold invertible; split; [unfold printable | unfold parsable]; 
+    compute [snd fst]; intros.
+    - repeat match goal with
+               | [v: [| Sum_t _ _ |] |- _ ] => case v as [v | v]
+               | [v: [| unit_t |] |- _] => destruct v
+               | [v:[|pair_t _ _|] |- _] => destruct v
+             end; abstract printable_tac.
+    - abstract (destruct w; parsable_tac).
+  Defined.
+
+  (* Inductive s_instr2 : Set := *)
+  (* | S_SHUFPS (op1 op2: sse_operand) (imm:int8) *)
+  (* | S_SQRTPS (op1 op2: sse_operand) *)
+  (* | S_SQRTSS (op1 op2: sse_operand) *)
+  (* | S_STMXCSR (op1 : sse_operand) *)
+  (* | S_SUBPS (op1 op2: sse_operand) *)
+  (* | S_SUBSS (op1 op2: sse_operand) *)
+  (* | S_UCOMISS (op1 op2: sse_operand) *)
+  (* | S_UNPCKHPS (op1 op2: sse_operand) *)
+  (* | S_UNPCKLPS (op1 op2: sse_operand) *)
+  (* | S_XORPS (op1 op2: sse_operand) *)
+  (* | S_PAVGB (op1 op2: sse_operand) *)
+  (* | S_PEXTRW (op1 op2: sse_operand) (imm:int8) *)
+  (* | S_PINSRW (op1 op2: sse_operand) (imm:int8) *)
+  (* | S_PMAXSW (op1 op2: sse_operand) *)
+  (* | S_PMAXUB (op1 op2: sse_operand) *)
+  (* | S_PMINSW (op1 op2: sse_operand) *)
+  (* | S_PMINUB (op1 op2: sse_operand) *)
+  (* | S_PMOVMSKB (op1 op2: sse_operand) *)
+  (* | S_PSADBW (op1 op2: sse_operand) *)
+  (* | S_PSHUFW (op1 op2: sse_operand) (imm:int8) *)
+  (* | S_MASKMOVQ (op1 op2: sse_operand) *)
+  (* | S_MOVNTPS (op1 op2: sse_operand) *)
+  (* | S_MOVNTQ (op1 op2: sse_operand) *)
+  (* | S_PREFETCHT0 (op1: sse_operand) *)
+  (* | S_PREFETCHT1 (op1: sse_operand) *)
+  (* | S_PREFETCHT2 (op1: sse_operand) *)
+  (* | S_PREFETCHNTA (op1: sse_operand) *)
+  (* | S_SFENCE. *)
+
+  Definition instr_grammar_env : AST_Env (pair_t prefix_t instruction_t) :=
+    {0, prefix_grammar_only_seg_override $ i_instr1_p,
+        (fun v => 
+           let (pre,hi):=v in
+           let i := match hi with
+                      | I_AAA => AAA
+                      | I_AAD => AAD
+                      | I_AAM => AAM
+                      | I_AAS => AAS
+                      | I_CLC => CLC
+                      | I_CLD => CLD
+                      | I_CLI => CLI
+                      | I_CLTS => CLTS
+                      | I_CMC => CMC
+                      | I_CPUID => CPUID
+                      | I_DAA => DAA
+                      | I_DAS => DAS
+                      | I_HLT => HLT
+                      | I_INT => INT
+                      | I_INTO => INTO
+                      | I_INVD => INVD
+                      | I_IRET => IRET
+                      | I_LAHF => LAHF
+                      | I_LEAVE => LEAVE
+                      | I_POPA => POPA
+                      | I_POPF => POPF
+                      | I_PUSHA => PUSHA
+                      | I_PUSHF => PUSHF
+                      | I_RDMSR => RDMSR
+                      | I_RDPMC => RDPMC
+                      | I_RDTSC => RDTSC
+                      | I_RDTSCP => RDTSCP
+                      | I_RSM => RSM
+                      | I_SAHF => SAHF
+                      | I_STC => STC
+                      | I_STD => STD
+                      | I_STI => STI
+                      | I_UD2 => UD2
+                      | I_WBINVD => WBINVD
+                      | I_WRMSR => WRMSR
+                      | I_XLAT => XLAT
+                    end
+               in (pre,i) %% pair_t prefix_t instruction_t)} :::
+    {1, prefix_grammar_only_seg_override $ i_instr2_p,
+        (fun v => 
+           let (pre,hi):=v in
+           let i := match hi with
+                      | I_ARPL op1 op2 => ARPL op1 op2
+                      | I_BOUND op1 op2 => BOUND op1 op2
+                      | I_BSF op1 op2 => BSF op1 op2
+                      | I_BSR op1 op2 => BSR op1 op2
+                      | I_BSWAP r => BSWAP r
+                      | I_BT op1 op2 => BT op1 op2
+                      | I_CALL near abs op sel => CALL near abs op sel
+                      | I_IN w p => IN w p
+                      | I_INTn it => INTn it
+                      | I_INVLPG op => INVLPG op
+                      | I_Jcc ct disp => Jcc ct disp
+                      | I_JCXZ b => JCXZ b
+                      | I_JMP near abs op sel => JMP near abs op sel
+                      | I_LAR op1 op2 => LAR op1 op2
+                      | I_LDS op1 op2 => LDS op1 op2
+                      | I_LEA op1 op2 => LEA op1 op2
+                      | I_LES op1 op2 => LES op1 op2
+                      | I_LFS op1 op2 => LFS op1 op2
+                      | I_LGDT op => LGDT op
+                      | I_LGS op1 op2 => LGS op1 op2
+                      | I_LIDT op => LIDT op
+                      | I_LLDT op => LLDT op
+                      | I_LMSW op => LMSW op
+                      | I_LOOP disp => LOOP disp
+                      | I_LOOPZ disp => LOOPZ disp
+                      | I_LOOPNZ disp => LOOPNZ disp
+                      | I_LSL op1 op2 => LSL op1 op2
+                      | I_LSS op1 op2 => LSS op1 op2
+                      | I_LTR op => LTR op
+                    end
+               in (pre,i) %% pair_t prefix_t instruction_t)} :::
+    {2, prefix_grammar_only_seg_override $ i_instr3_p,
+        (fun v => 
+           let (pre,hi):=v in
+           let i := match hi with
+                      | I_MOVCR d cr r => MOVCR d cr r
+                      | I_MOVDR d cr r => MOVDR d cr r
+                      | I_MOVSR d cr r => MOVSR d cr r
+                      | I_MOVBE op1 op2 => MOVBE op1 op2
+                      | I_OUT w p => OUT w p
+                      | I_POP op => POP op
+                      | I_POPSR sr => POPSR sr
+                      | I_PUSH w op => PUSH w op
+                      | I_PUSHSR sr => PUSHSR sr
+                      | I_RCL w op1 ri => RCL w op1 ri
+                      | I_RCR w op1 ri => RCR w op1 ri
+                      | I_SETcc ct op => SETcc ct op
+                      | I_SGDT op => SGDT op
+                      | I_SIDT op => SIDT op
+                      | I_SLDT op => SLDT op
+                      | I_SMSW op => SMSW op
+                      | I_STR op => STR op
+                      | I_VERR op => VERR op
+                      | I_VERW op => VERW op
+                    end
+               in (pre,i) %% pair_t prefix_t instruction_t)} :::
+    {3, i_instr4_grammar,
+        (fun v => 
+           let (pre,hi):=v in
+           let i := match hi with
+                      | I_INS b => INS b
+                      | I_OUTS b => OUTS b
+                      | I_MOVS b => MOVS b
+                      | I_LODS b => LODS b
+                      | I_STOS b => STOS b
+                      | I_RET ss disp => RET ss disp
+                      | I_CMPS b => CMPS b
+                      | I_SCAS b => SCAS b
+                    end
+               in (pre,i) %% pair_t prefix_t instruction_t)} :::
+    {4, i_instr5_grammar,
+        (fun v => 
+           let (pre,hi):=v in
+           let i := match hi with
+                      | I_ADC w op1 op2 => ADC w op1 op2
+                      | I_ADD w op1 op2 => ADD w op1 op2
+                      | I_AND w op1 op2 => AND w op1 op2
+                      | I_BTC op1 op2 => BTC op1 op2
+                      | I_BTR op1 op2 => BTR op1 op2
+                      | I_BTS op1 op2 => BTS op1 op2
+                      | I_CMP w op1 op2 => CMP w op1 op2
+                      | I_CMPXCHG w op1 op2 => CMPXCHG w op1 op2
+                      | I_DEC w op1 => DEC w op1
+                      | I_IMUL w op1 opopt iopt  => IMUL w op1 opopt iopt
+                      | I_INC w op1 => INC w op1
+                      | I_MOV w op1 op2 => MOV w op1 op2
+                      | I_NEG w op => NEG w op
+                      | I_NOT w op => NOT w op
+                      | I_OR w op1 op2 => OR w op1 op2
+                      | I_SBB w op1 op2 => SBB w op1 op2
+                      | I_SUB w op1 op2 => SUB w op1 op2
+                      | I_TEST w op1 op2 => TEST w op1 op2
+                      | I_XADD w op1 op2 => XADD w op1 op2
+                      | I_XCHG w op1 op2 => XCHG w op1 op2
+                      | I_XOR w op1 op2 => XOR w op1 op2
+                    end
+               in (pre,i) %% pair_t prefix_t instruction_t)} :::
+    {5, prefix_grammar_seg_op_override $ i_instr6_p,
+        (fun v => 
+           let (pre,hi):=v in
+           let i := match hi with
+                      | I_CDQ => CDQ
+                      | I_CMOVcc ct op1 op2 => CMOVcc ct op1 op2
+                      | I_CWDE => CWDE
+                      | I_DIV w op1 => DIV w op1
+                      | I_IDIV w op1 => IDIV w op1
+                      | I_MOVSX w op1 op2 => MOVSX w op1 op2
+                      | I_MOVZX w op1 op2 => MOVZX w op1 op2
+                      | I_MUL w op1 => MUL w op1
+                      | I_NOP op => NOP op
+                      | I_ROL w op1 ri => ROL w op1 ri
+                      | I_ROR w op1 ri => ROR w op1 ri
+                      | I_SAR w op1 ri => SAR w op1 ri
+                      | I_SHL w op1 ri => SHL w op1 ri
+                      | I_SHLD op1 r ri => SHLD op1 r ri
+                      | I_SHR w op1 ri => SHR w op1 ri
+                      | I_SHRD op1 r ri => SHRD op1 r ri
+                    end
+               in (pre,i) %% pair_t prefix_t instruction_t)} :::
+    {6, prefix_grammar_only_seg_override $ f_instr1_p,
+        (fun v => 
+           let (pre,hi):=v in
+           let i := match hi with
+                      | F_F2XM1 => F2XM1
+                      | F_FABS => FABS
+                      | F_FADD z op1 => FADD z op1
+                      | F_FADDP op => FADDP op
+                      | F_FBLD op => FBLD op
+                      | F_FBSTP op => FBSTP op
+                      | F_FCHS => FCHS
+                      | F_FCMOVcc ct op => FCMOVcc ct op
+                      | F_FCOM op => FCOM op
+                      | F_FCOMP op => FCOMP op
+                      | F_FCOMPP => FCOMPP
+                      | F_FCOMIP op => FCOMIP op
+                      | F_FCOS => FCOS
+                      | F_FDECSTP => FDECSTP
+                      | F_FDIV z op => FDIV z op
+                      | F_FDIVP op => FDIVP op
+                      | F_FDIVR z op => FDIVR z op
+                      | F_FDIVRP op => FDIVRP op
+                      | F_FFREE op => FFREE op
+                      | F_FIADD op => FIADD op
+                      | F_FICOM op => FICOM op
+                      | F_FICOMP op => FICOMP op
+                      | F_FIDIV op => FIDIV op
+                      | F_FIDIVR op => FIDIVR op
+                      | F_FILD op => FILD op
+                      | F_FIMUL op => FIMUL op
+                      | F_FINCSTP => FINCSTP
+                      | F_FIST op => FIST op
+                      | F_FISTP op => FISTP op
+                      | F_FISUB op => FISUB op
+                      | F_FISUBR op => FISUBR op
+                      | F_FLD op => FLD op
+                      | F_FLD1 => FLD1
+                      | F_FLDCW op => FLDCW op
+                      | F_FLDENV op => FLDENV op
+                      | F_FLDL2E => FLDL2E
+                      | F_FLDL2T => FLDL2T
+                      | F_FLDLG2 => FLDLG2
+                      | F_FLDLN2 => FLDLN2
+                      | F_FLDPI => FLDPI
+                      | F_FLDZ => FLDZ
+                      | F_FMUL z op => FMUL z op
+                      | F_FMULP op => FMULP op
+                    end
+               in (pre,i) %% pair_t prefix_t instruction_t)} :::
+    {7, prefix_grammar_only_seg_override $ f_instr2_p,
+        (fun v => 
+           let (pre,hi):=v in
+           let i := match hi with
+                      | F_FNCLEX => FNCLEX
+                      | F_FNINIT => FNINIT
+                      | F_FNOP => FNOP
+                      | F_FNSAVE op => FNSAVE op
+                      | F_FNSTCW op => FNSTCW op
+                      | F_FNSTSW op => FNSTSW op
+                      | F_FPATAN => FPATAN
+                      | F_FPREM => FPREM
+                      | F_FPREM1 => FPREM1
+                      | F_FPTAN => FPTAN
+                      | F_FRNDINT => FRNDINT
+                      | F_FRSTOR op => FRSTOR op
+                      | F_FSCALE => FSCALE
+                      | F_FSIN => FSIN
+                      | F_FSINCOS => FSINCOS
+                      | F_FSQRT => FSQRT
+                      | F_FST op => FST op
+                      | F_FSTENV op => FSTENV op
+                      | F_FSTP op => FSTP op
+                      | F_FSUB z op => FSUB z op
+                      | F_FSUBP op => FSUBP op
+                      | F_FSUBR z op => FSUBR z op
+                      | F_FSUBRP op => FSUBRP op
+                      | F_FTST => FTST
+                      | F_FUCOM op => FUCOM op
+                      | F_FUCOMP op => FUCOMP op
+                      | F_FUCOMPP => FUCOMPP
+                      | F_FUCOMI op => FUCOMI op
+                      | F_FUCOMIP op => FUCOMIP op
+                      | F_FXAM => FXAM
+                      | F_FXCH op => FXCH op
+                      | F_FXTRACT => FXTRACT
+                      | F_FYL2X => FYL2X
+                      | F_FYL2XP1 => FYL2XP1
+                      | F_FWAIT => FWAIT
+                    end
+               in (pre,i) %% pair_t prefix_t instruction_t)} :::
+    {8, prefix_grammar_only_seg_override $ m_instr_p,
+        (fun v => 
+           let (pre,hi):=v in
+           let i := match hi with
+                      | M_EMMS => EMMS
+                      | M_MOVD op1 op2 => MOVD op1 op2
+                      | M_MOVQ op1 op2 => MOVQ op1 op2
+                      | M_PACKSSDW op1 op2 => PACKSSDW op1 op2
+                      | M_PACKSSWB op1 op2 => PACKSSWB op1 op2
+                      | M_PACKUSWB op1 op2 => PACKUSWB op1 op2
+                      | M_PADD gg op1 op2 => PADD gg op1 op2
+                      | M_PADDS gg op1 op2 => PADDS gg op1 op2
+                      | M_PADDUS gg op1 op2 => PADDUS gg op1 op2
+                      | M_PAND op1 op2 => PAND op1 op2
+                      | M_PANDN op1 op2 => PANDN op1 op2
+                      | M_PCMPEQ gg op1 op2 => PCMPEQ gg op1 op2
+                      | M_PCMPGT gg op1 op2 => PCMPGT gg op1 op2
+                      | M_PMADDWD op1 op2 => PMADDWD op1 op2
+                      | M_PMULHUW op1 op2 => PMULHUW op1 op2
+                      | M_PMULHW op1 op2 => PMULHW op1 op2
+                      | M_PMULLW op1 op2 => PMULLW op1 op2
+                      | M_POR op1 op2 => POR op1 op2
+                      | M_PSLL gg op1 op2 => PSLL gg op1 op2
+                      | M_PSRA gg op1 op2 => PSRA gg op1 op2
+                      | M_PSRL gg op1 op2 => PSRL gg op1 op2
+                      | M_PSUB gg op1 op2 => PSUB gg op1 op2
+                      | M_PSUBS gg op1 op2 => PSUBS gg op1 op2
+                      | M_PSUBUS gg op1 op2 => PSUBUS gg op1 op2
+                      | M_PUNPCKH gg op1 op2 => PUNPCKH gg op1 op2
+                      | M_PUNPCKL gg op1 op2 => PUNPCKL gg op1 op2
+                      | M_PXOR op1 op2 => PXOR op1 op2
+                    end
+               in (pre,i) %% pair_t prefix_t instruction_t)} :::
+    {9, prefix_grammar_only_seg_override $ s_instr1_p,
+        (fun v => 
+           let (pre,hi):=v in
+           let i := match hi with
+                      | S_ADDPS op1 op2 => ADDPS op1 op2
+                      | S_ADDSS op1 op2 => ADDSS op1 op2
+                      | S_ANDNPS op1 op2 => ANDNPS op1 op2
+                      | S_ANDPS op1 op2 => ANDPS op1 op2
+                      | S_CMPPS op1 op2 imm => CMPPS op1 op2 imm
+                      | S_CMPSS op1 op2 imm => CMPSS op1 op2 imm
+                      | S_COMISS op1 op2 => COMISS op1 op2
+                      | S_CVTPI2PS op1 op2 => CVTPI2PS op1 op2
+                      | S_CVTPS2PI op1 op2 => CVTPS2PI op1 op2
+                      | S_CVTSI2SS op1 op2 => CVTSI2SS op1 op2
+                      | S_CVTSS2SI op1 op2 => CVTSS2SI op1 op2
+                      | S_CVTTPS2PI op1 op2 => CVTTPS2PI op1 op2
+                      | S_CVTTSS2SI op1 op2 => CVTTSS2SI op1 op2
+                      | S_DIVPS op1 op2 => DIVPS op1 op2
+                      | S_DIVSS op1 op2 => DIVSS op1 op2
+                      | S_LDMXCSR op => LDMXCSR op
+                      | S_MAXPS op1 op2 => MAXPS op1 op2
+                      | S_MAXSS op1 op2 => MAXSS op1 op2
+                      | S_MINPS op1 op2 => MINPS op1 op2
+                      | S_MINSS op1 op2 => MINSS op1 op2
+                      | S_MOVAPS op1 op2 => MOVAPS op1 op2
+                      | S_MOVHLPS op1 op2 => MOVHLPS op1 op2
+                      | S_MOVHPS op1 op2 => MOVHPS op1 op2
+                      | S_MOVLHPS op1 op2 => MOVLHPS op1 op2
+                      | S_MOVLPS op1 op2 => MOVLPS op1 op2
+                      | S_MOVMSKPS op1 op2 => MOVMSKPS op1 op2
+                      | S_MOVSS op1 op2 => MOVSS op1 op2
+                      | S_MOVUPS op1 op2 => MOVUPS op1 op2
+                      | S_MULPS op1 op2 => MULPS op1 op2
+                      | S_MULSS op1 op2 => MULSS op1 op2
+                      | S_ORPS op1 op2 => ORPS op1 op2
+                      | S_RCPPS op1 op2 => RCPPS op1 op2
+                      | S_RCPSS op1 op2 => RCPSS op1 op2
+                      | S_RSQRTPS op1 op2 => RSQRTPS op1 op2
+                      | S_RSQRTSS op1 op2 => RSQRTSS op1 op2
+                    end
+               in (pre,i) %% pair_t prefix_t instruction_t)} :::
+    {10, prefix_grammar_only_seg_override $ s_instr2_p,
+        (fun v => 
+           let (pre,hi):=v in
+           let i := match hi with
+                      | S_SHUFPS op1 op2 imm => SHUFPS op1 op2 imm
+                      | S_SQRTPS op1 op2 => SQRTPS op1 op2
+                      | S_SQRTSS op1 op2 => SQRTSS op1 op2
+                      | S_STMXCSR op => STMXCSR op
+                      | S_SUBPS op1 op2 => SUBPS op1 op2
+                      | S_SUBSS op1 op2 => SUBSS op1 op2
+                      | S_UCOMISS op1 op2 => UCOMISS op1 op2
+                      | S_UNPCKHPS op1 op2 => UNPCKHPS op1 op2
+                      | S_UNPCKLPS op1 op2 => UNPCKLPS op1 op2
+                      | S_XORPS op1 op2 => XORPS op1 op2
+                      | S_PAVGB op1 op2 => PAVGB op1 op2
+                      | S_PEXTRW op1 op2 imm => PEXTRW op1 op2 imm
+                      | S_PINSRW op1 op2 imm => PINSRW op1 op2 imm
+                      | S_PMAXSW op1 op2 => PMAXSW op1 op2
+                      | S_PMAXUB op1 op2 => PMAXUB op1 op2
+                      | S_PMINSW op1 op2 => PMINSW op1 op2
+                      | S_PMINUB op1 op2 => PMINUB op1 op2
+                      | S_PMOVMSKB op1 op2 => PMOVMSKB op1 op2
+                      | S_PSADBW op1 op2 => PSADBW op1 op2
+                      | S_PSHUFW op1 op2 imm => PSHUFW op1 op2 imm
+                      | S_MASKMOVQ op1 op2 => MASKMOVQ op1 op2
+                      | S_MOVNTPS op1 op2 => MOVNTPS op1 op2
+                      | S_MOVNTQ op1 op2 => MOVNTQ op1 op2
+                      | S_PREFETCHT0 op => PREFETCHT0 op
+                      | S_PREFETCHT1 op => PREFETCHT1 op
+                      | S_PREFETCHT2 op => PREFETCHT2 op
+                      | S_PREFETCHNTA op => PREFETCHNTA op
+                      | S_SFENCE => SFENCE
+                    end
+               in (pre,i) %% pair_t prefix_t instruction_t)} :::
+    ast_env_nil.
+  Hint Unfold instr_grammar_env: env_unfold_db.
+
+  Definition instruction_grammar : wf_bigrammar (pair_t prefix_t instruction_t).
+    gen_ast_defs instr_grammar_env.
+    refine (gr @ (mp: _ -> [|pair_t prefix_t instruction_t|])
+               & (fun u:[|pair_t prefix_t instruction_t|] =>
+                   let (pre,i):=u in
+                   match i with
+                     | AAA => case0 (pre,I_AAA)
+                     | AAD => case0 (pre,I_AAD)
+                     | AAM => case0 (pre,I_AAM)
+                     | AAS => case0 (pre,I_AAS)
+                     | CLC => case0 (pre,I_CLC)
+                     | CLD => case0 (pre,I_CLD)
+                     | CLI => case0 (pre,I_CLI)
+                     | CLTS => case0 (pre,I_CLTS)
+                     | CMC => case0 (pre,I_CMC)
+                     | CPUID => case0 (pre,I_CPUID)
+                     | DAA => case0 (pre,I_DAA)
+                     | DAS => case0 (pre,I_DAS)
+                     | HLT => case0 (pre,I_HLT)
+                     | INT => case0 (pre,I_INT)
+                     | INTO => case0 (pre,I_INTO)
+                     | INVD => case0 (pre,I_INVD)
+                     | IRET => case0 (pre,I_IRET)
+                     | LAHF => case0 (pre,I_LAHF)
+                     | LEAVE => case0 (pre,I_LEAVE)
+                     | POPA => case0 (pre,I_POPA)
+                     | POPF => case0 (pre,I_POPF)
+                     | PUSHA => case0 (pre,I_PUSHA)
+                     | PUSHF => case0 (pre,I_PUSHF)
+                     | RDMSR => case0 (pre,I_RDMSR)
+                     | RDPMC => case0 (pre,I_RDPMC)
+                     | RDTSC => case0 (pre,I_RDTSC)
+                     | RDTSCP => case0 (pre,I_RDTSCP)
+                     | RSM => case0 (pre,I_RSM)
+                     | SAHF => case0 (pre,I_SAHF)
+                     | STC => case0 (pre,I_STC)
+                     | STD => case0 (pre,I_STD)
+                     | STI => case0 (pre,I_STI)
+                     | UD2 => case0 (pre,I_UD2)
+                     | WBINVD => case0 (pre,I_WBINVD)
+                     | WRMSR => case0 (pre,I_WRMSR)
+                     | XLAT => case0 (pre,I_XLAT)
+
+                     | ARPL op1 op2 => case1 (pre,I_ARPL op1 op2)
+                     | BOUND op1 op2 => case1 (pre,I_BOUND op1 op2)
+                     | BSF op1 op2 => case1 (pre,I_BSF op1 op2)
+                     | BSR op1 op2 => case1 (pre,I_BSR op1 op2)
+                     | BSWAP r => case1 (pre,I_BSWAP r)
+                     | BT op1 op2 => case1 (pre,I_BT op1 op2)
+                     | CALL near abs op sel => case1 (pre,I_CALL near abs op sel)
+                     | IN w p => case1 (pre,I_IN w p)
+                     | INTn it => case1 (pre,I_INTn it)
+                     | INVLPG op => case1 (pre,I_INVLPG op)
+                     | Jcc ct disp => case1 (pre,I_Jcc ct disp)
+                     | JCXZ b => case1 (pre,I_JCXZ b)
+                     | JMP near abs op sel => case1 (pre,I_JMP near abs op sel)
+                     | LAR op1 op2 => case1 (pre,I_LAR op1 op2)
+                     | LDS op1 op2 => case1 (pre,I_LDS op1 op2)
+                     | LEA op1 op2 => case1 (pre,I_LEA op1 op2)
+                     | LES op1 op2 => case1 (pre,I_LES op1 op2)
+                     | LFS op1 op2 => case1 (pre,I_LFS op1 op2)
+                     | LGDT op => case1 (pre,I_LGDT op)
+                     | LGS op1 op2 => case1 (pre,I_LGS op1 op2)
+                     | LIDT op => case1 (pre,I_LIDT op)
+                     | LLDT op => case1 (pre,I_LLDT op)
+                     | LMSW op => case1 (pre,I_LMSW op)
+                     | LOOP disp => case1 (pre,I_LOOP disp)
+                     | LOOPZ disp => case1 (pre,I_LOOPZ disp)
+                     | LOOPNZ disp => case1 (pre,I_LOOPNZ disp)
+                     | LSL op1 op2 => case1 (pre,I_LSL op1 op2)
+                     | LSS op1 op2 => case1 (pre,I_LSS op1 op2)
+                     | LTR op => case1 (pre,I_LTR op)
+
+                     | MOVCR d cr r => case2 (pre,I_MOVCR d cr r)
+                     | MOVDR d cr r => case2 (pre,I_MOVDR d cr r)
+                     | MOVSR d cr r => case2 (pre,I_MOVSR d cr r)
+                     | MOVBE op1 op2 => case2 (pre,I_MOVBE op1 op2)
+                     | OUT w p => case2 (pre,I_OUT w p)
+                     | POP op => case2 (pre,I_POP op)
+                     | POPSR sr => case2 (pre,I_POPSR sr)
+                     | PUSH w op => case2 (pre,I_PUSH w op)
+                     | PUSHSR sr => case2 (pre,I_PUSHSR sr)
+                     | RCL w op1 ri => case2 (pre,I_RCL w op1 ri)
+                     | RCR w op1 ri => case2 (pre,I_RCR w op1 ri)
+                     | SETcc ct op => case2 (pre,I_SETcc ct op)
+                     | SGDT op => case2 (pre,I_SGDT op)
+                     | SIDT op => case2 (pre,I_SIDT op)
+                     | SLDT op => case2 (pre,I_SLDT op)
+                     | SMSW op => case2 (pre,I_SMSW op)
+                     | STR op => case2 (pre,I_STR op)
+                     | VERR op => case2 (pre,I_VERR op)
+                     | VERW op => case2 (pre,I_VERW op)
+                                          
+                     | INS b => case3 (pre,I_INS b)
+                     | OUTS b => case3 (pre,I_OUTS b)
+                     | MOVS b => case3 (pre,I_MOVS b)
+                     | LODS b => case3 (pre,I_LODS b)
+                     | STOS b => case3 (pre,I_STOS b)
+                     | RET ss disp => case3 (pre,I_RET ss disp)
+                     | CMPS b => case3 (pre,I_CMPS b)
+                     | SCAS b => case3 (pre,I_SCAS b)
+
+                     | ADC w op1 op2 => case4 (pre, I_ADC w op1 op2)
+                     | ADD w op1 op2 => case4 (pre, I_ADD w op1 op2)
+                     | AND w op1 op2 => case4 (pre, I_AND w op1 op2)
+                     | BTC op1 op2 => case4 (pre, I_BTC op1 op2)
+                     | BTR op1 op2 => case4 (pre, I_BTR op1 op2)
+                     | BTS op1 op2 => case4 (pre, I_BTS op1 op2)
+                     | CMP w op1 op2 => case4 (pre, I_CMP w op1 op2)
+                     | CMPXCHG w op1 op2 => case4 (pre, I_CMPXCHG w op1 op2)
+                     | DEC w op1 => case4 (pre, I_DEC w op1)
+                     | IMUL w op1 opopt iopt  => case4 (pre, I_IMUL w op1 opopt iopt)
+                     | INC w op1 => case4 (pre, I_INC w op1)
+                     | MOV w op1 op2 => case4 (pre, I_MOV w op1 op2)
+                     | NEG w op => case4 (pre, I_NEG w op)
+                     | NOT w op => case4 (pre, I_NOT w op)
+                     | OR w op1 op2 => case4 (pre, I_OR w op1 op2)
+                     | SBB w op1 op2 => case4 (pre, I_SBB w op1 op2)
+                     | SUB w op1 op2 => case4 (pre, I_SUB w op1 op2)
+                     | TEST w op1 op2 => case4 (pre, I_TEST w op1 op2)
+                     | XADD w op1 op2 => case4 (pre, I_XADD w op1 op2)
+                     | XCHG w op1 op2 => case4 (pre, I_XCHG w op1 op2)
+                     | XOR w op1 op2 => case4 (pre, I_XOR w op1 op2)
+
+                     | CDQ => case5 (pre, I_CDQ)
+                     | CMOVcc ct op1 op2 => case5 (pre, I_CMOVcc ct op1 op2)
+                     | CWDE => case5 (pre, I_CWDE)
+                     | DIV w op1 => case5 (pre, I_DIV w op1)
+                     | IDIV w op1 => case5 (pre, I_IDIV w op1)
+                     | MOVSX w op1 op2 => case5 (pre, I_MOVSX w op1 op2)
+                     | MOVZX w op1 op2 => case5 (pre, I_MOVZX w op1 op2)
+                     | MUL w op1 => case5 (pre, I_MUL w op1)
+                     | NOP op => case5 (pre, I_NOP op)
+                     | ROL w op1 ri => case5 (pre, I_ROL w op1 ri)
+                     | ROR w op1 ri => case5 (pre, I_ROR w op1 ri)
+                     | SAR w op1 ri => case5 (pre, I_SAR w op1 ri)
+                     | SHL w op1 ri => case5 (pre, I_SHL w op1 ri)
+                     | SHLD op1 r ri => case5 (pre, I_SHLD op1 r ri)
+                     | SHR w op1 ri => case5 (pre, I_SHR w op1 ri)
+                     | SHRD op1 r ri => case5 (pre, I_SHRD op1 r ri)
+
+                     | F2XM1 => case6 (pre, F_F2XM1)
+                     | FABS => case6 (pre, F_FABS)
+                     | FADD z op1 => case6 (pre, F_FADD z op1)
+                     | FADDP op => case6 (pre, F_FADDP op)
+                     | FBLD op => case6 (pre, F_FBLD op)
+                     | FBSTP op => case6 (pre, F_FBSTP op)
+                     | FCHS => case6 (pre, F_FCHS)
+                     | FCMOVcc ct op => case6 (pre, F_FCMOVcc ct op)
+                     | FCOM op => case6 (pre, F_FCOM op)
+                     | FCOMP op => case6 (pre, F_FCOMP op)
+                     | FCOMPP => case6 (pre, F_FCOMPP)
+                     | FCOMIP op => case6 (pre, F_FCOMIP op)
+                     | FCOS => case6 (pre, F_FCOS)
+                     | FDECSTP => case6 (pre, F_FDECSTP)
+                     | FDIV z op => case6 (pre, F_FDIV z op)
+                     | FDIVP op => case6 (pre, F_FDIVP op)
+                     | FDIVR z op => case6 (pre, F_FDIVR z op)
+                     | FDIVRP op => case6 (pre, F_FDIVRP op)
+                     | FFREE op => case6 (pre, F_FFREE op)
+                     | FIADD op => case6 (pre, F_FIADD op)
+                     | FICOM op => case6 (pre, F_FICOM op)
+                     | FICOMP op => case6 (pre, F_FICOMP op)
+                     | FIDIV op => case6 (pre, F_FIDIV op)
+                     | FIDIVR op => case6 (pre, F_FIDIVR op)
+                     | FILD op => case6 (pre, F_FILD op)
+                     | FIMUL op => case6 (pre, F_FIMUL op)
+                     | FINCSTP => case6 (pre, F_FINCSTP)
+                     | FIST op => case6 (pre, F_FIST op)
+                     | FISTP op => case6 (pre, F_FISTP op)
+                     | FISUB op => case6 (pre, F_FISUB op)
+                     | FISUBR op => case6 (pre, F_FISUBR op)
+                     | FLD op => case6 (pre, F_FLD op)
+                     | FLD1 => case6 (pre, F_FLD1)
+                     | FLDCW op => case6 (pre, F_FLDCW op)
+                     | FLDENV op => case6 (pre, F_FLDENV op)
+                     | FLDL2E => case6 (pre, F_FLDL2E)
+                     | FLDL2T => case6 (pre, F_FLDL2T)
+                     | FLDLG2 => case6 (pre, F_FLDLG2)
+                     | FLDLN2 => case6 (pre, F_FLDLN2)
+                     | FLDPI => case6 (pre, F_FLDPI)
+                     | FLDZ => case6 (pre, F_FLDZ)
+                     | FMUL z op => case6 (pre, F_FMUL z op)
+                     | FMULP op => case6 (pre, F_FMULP op)
+
+                     | FNCLEX => case7 (pre, F_FNCLEX)
+                     | FNINIT => case7 (pre, F_FNINIT)
+                     | FNOP => case7 (pre, F_FNOP)
+                     | FNSAVE op => case7 (pre, F_FNSAVE op)
+                     | FNSTCW op => case7 (pre, F_FNSTCW op)
+                     | FNSTSW op => case7 (pre, F_FNSTSW op)
+                     | FPATAN => case7 (pre, F_FPATAN)
+                     | FPREM => case7 (pre, F_FPREM)
+                     | FPREM1 => case7 (pre, F_FPREM1)
+                     | FPTAN => case7 (pre, F_FPTAN)
+                     | FRNDINT => case7 (pre, F_FRNDINT)
+                     | FRSTOR op => case7 (pre, F_FRSTOR op)
+                     | FSCALE => case7 (pre, F_FSCALE)
+                     | FSIN => case7 (pre, F_FSIN)
+                     | FSINCOS => case7 (pre, F_FSINCOS)
+                     | FSQRT => case7 (pre, F_FSQRT)
+                     | FST op => case7 (pre, F_FST op)
+                     | FSTENV op => case7 (pre, F_FSTENV op)
+                     | FSTP op => case7 (pre, F_FSTP op)
+                     | FSUB z op => case7 (pre, F_FSUB z op)
+                     | FSUBP op => case7 (pre, F_FSUBP op)
+                     | FSUBR z op => case7 (pre, F_FSUBR z op)
+                     | FSUBRP op => case7 (pre, F_FSUBRP op)
+                     | FTST => case7 (pre, F_FTST)
+                     | FUCOM op => case7 (pre, F_FUCOM op)
+                     | FUCOMP op => case7 (pre, F_FUCOMP op)
+                     | FUCOMPP => case7 (pre, F_FUCOMPP)
+                     | FUCOMI op => case7 (pre, F_FUCOMI op)
+                     | FUCOMIP op => case7 (pre, F_FUCOMIP op)
+                     | FXAM => case7 (pre, F_FXAM)
+                     | FXCH op => case7 (pre, F_FXCH op)
+                     | FXTRACT => case7 (pre, F_FXTRACT)
+                     | FYL2X => case7 (pre, F_FYL2X)
+                     | FYL2XP1 => case7 (pre, F_FYL2XP1)
+                     | FWAIT => case7 (pre, F_FWAIT)
+
+                     | EMMS => case8 (pre, M_EMMS)
+                     | MOVD op1 op2 => case8 (pre, M_MOVD op1 op2)
+                     | MOVQ op1 op2 => case8 (pre, M_MOVQ op1 op2)
+                     | PACKSSDW op1 op2 => case8 (pre, M_PACKSSDW op1 op2)
+                     | PACKSSWB op1 op2 => case8 (pre, M_PACKSSWB op1 op2)
+                     | PACKUSWB op1 op2 => case8 (pre, M_PACKUSWB op1 op2)
+                     | PADD gg op1 op2 => case8 (pre, M_PADD gg op1 op2)
+                     | PADDS gg op1 op2 => case8 (pre, M_PADDS gg op1 op2)
+                     | PADDUS gg op1 op2 => case8 (pre, M_PADDUS gg op1 op2)
+                     | PAND op1 op2 => case8 (pre, M_PAND op1 op2)
+                     | PANDN op1 op2 => case8 (pre, M_PANDN op1 op2)
+                     | PCMPEQ gg op1 op2 => case8 (pre, M_PCMPEQ gg op1 op2)
+                     | PCMPGT gg op1 op2 => case8 (pre, M_PCMPGT gg op1 op2)
+                     | PMADDWD op1 op2 => case8 (pre, M_PMADDWD op1 op2)
+                     | PMULHUW op1 op2 => case8 (pre, M_PMULHUW op1 op2)
+                     | PMULHW op1 op2 => case8 (pre, M_PMULHW op1 op2)
+                     | PMULLW op1 op2 => case8 (pre, M_PMULLW op1 op2)
+                     | POR op1 op2 => case8 (pre, M_POR op1 op2)
+                     | PSLL gg op1 op2 => case8 (pre, M_PSLL gg op1 op2)
+                     | PSRA gg op1 op2 => case8 (pre, M_PSRA gg op1 op2)
+                     | PSRL gg op1 op2 => case8 (pre, M_PSRL gg op1 op2)
+                     | PSUB gg op1 op2 => case8 (pre, M_PSUB gg op1 op2)
+                     | PSUBS gg op1 op2 => case8 (pre, M_PSUBS gg op1 op2)
+                     | PSUBUS gg op1 op2 => case8 (pre, M_PSUBUS gg op1 op2)
+                     | PUNPCKH gg op1 op2 => case8 (pre, M_PUNPCKH gg op1 op2)
+                     | PUNPCKL gg op1 op2 => case8 (pre, M_PUNPCKL gg op1 op2)
+                     | PXOR op1 op2 => case8 (pre, M_PXOR op1 op2)
+
+                     | ADDPS op1 op2 => case9 (pre, S_ADDPS op1 op2)
+                     | ADDSS op1 op2 => case9 (pre, S_ADDSS op1 op2)
+                     | ANDNPS op1 op2 => case9 (pre, S_ANDNPS op1 op2)
+                     | ANDPS op1 op2 => case9 (pre, S_ANDPS op1 op2)
+                     | CMPPS op1 op2 imm => case9 (pre, S_CMPPS op1 op2 imm)
+                     | CMPSS op1 op2 imm => case9 (pre, S_CMPSS op1 op2 imm)
+                     | COMISS op1 op2 => case9 (pre, S_COMISS op1 op2)
+                     | CVTPI2PS op1 op2 => case9 (pre, S_CVTPI2PS op1 op2)
+                     | CVTPS2PI op1 op2 => case9 (pre, S_CVTPS2PI op1 op2)
+                     | CVTSI2SS op1 op2 => case9 (pre, S_CVTSI2SS op1 op2)
+                     | CVTSS2SI op1 op2 => case9 (pre, S_CVTSS2SI op1 op2)
+                     | CVTTPS2PI op1 op2 => case9 (pre, S_CVTTPS2PI op1 op2)
+                     | CVTTSS2SI op1 op2 => case9 (pre, S_CVTTSS2SI op1 op2)
+                     | DIVPS op1 op2 => case9 (pre, S_DIVPS op1 op2)
+                     | DIVSS op1 op2 => case9 (pre, S_DIVSS op1 op2)
+                     | LDMXCSR op => case9 (pre, S_LDMXCSR op)
+                     | MAXPS op1 op2 => case9 (pre, S_MAXPS op1 op2)
+                     | MAXSS op1 op2 => case9 (pre, S_MAXSS op1 op2)
+                     | MINPS op1 op2 => case9 (pre, S_MINPS op1 op2)
+                     | MINSS op1 op2 => case9 (pre, S_MINSS op1 op2)
+                     | MOVAPS op1 op2 => case9 (pre, S_MOVAPS op1 op2)
+                     | MOVHLPS op1 op2 => case9 (pre, S_MOVHLPS op1 op2)
+                     | MOVHPS op1 op2 => case9 (pre, S_MOVHPS op1 op2)
+                     | MOVLHPS op1 op2 => case9 (pre, S_MOVLHPS op1 op2)
+                     | MOVLPS op1 op2 => case9 (pre, S_MOVLPS op1 op2)
+                     | MOVMSKPS op1 op2 => case9 (pre, S_MOVMSKPS op1 op2)
+                     | MOVSS op1 op2 => case9 (pre, S_MOVSS op1 op2)
+                     | MOVUPS op1 op2 => case9 (pre, S_MOVUPS op1 op2)
+                     | MULPS op1 op2 => case9 (pre, S_MULPS op1 op2)
+                     | MULSS op1 op2 => case9 (pre, S_MULSS op1 op2)
+                     | ORPS op1 op2 => case9 (pre, S_ORPS op1 op2)
+                     | RCPPS op1 op2 => case9 (pre, S_RCPPS op1 op2)
+                     | RCPSS op1 op2 => case9 (pre, S_RCPSS op1 op2)
+                     | RSQRTPS op1 op2 => case9 (pre, S_RSQRTPS op1 op2)
+                     | RSQRTSS op1 op2 => case9 (pre, S_RSQRTSS op1 op2)
+
+                     | SHUFPS op1 op2 imm => case10 (pre, S_SHUFPS op1 op2 imm)
+                     | SQRTPS op1 op2 => case10 (pre, S_SQRTPS op1 op2)
+                     | SQRTSS op1 op2 => case10 (pre, S_SQRTSS op1 op2)
+                     | STMXCSR op => case10 (pre, S_STMXCSR op)
+                     | SUBPS op1 op2 => case10 (pre, S_SUBPS op1 op2)
+                     | SUBSS op1 op2 => case10 (pre, S_SUBSS op1 op2)
+                     | UCOMISS op1 op2 => case10 (pre, S_UCOMISS op1 op2)
+                     | UNPCKHPS op1 op2 => case10 (pre, S_UNPCKHPS op1 op2)
+                     | UNPCKLPS op1 op2 => case10 (pre, S_UNPCKLPS op1 op2)
+                     | XORPS op1 op2 => case10 (pre, S_XORPS op1 op2)
+                     | PAVGB op1 op2 => case10 (pre, S_PAVGB op1 op2)
+                     | PEXTRW op1 op2 imm => case10 (pre, S_PEXTRW op1 op2 imm)
+                     | PINSRW op1 op2 imm => case10 (pre, S_PINSRW op1 op2 imm)
+                     | PMAXSW op1 op2 => case10 (pre, S_PMAXSW op1 op2)
+                     | PMAXUB op1 op2 => case10 (pre, S_PMAXUB op1 op2)
+                     | PMINSW op1 op2 => case10 (pre, S_PMINSW op1 op2)
+                     | PMINUB op1 op2 => case10 (pre, S_PMINUB op1 op2)
+                     | PMOVMSKB op1 op2 => case10 (pre, S_PMOVMSKB op1 op2)
+                     | PSADBW op1 op2 => case10 (pre, S_PSADBW op1 op2)
+                     | PSHUFW op1 op2 imm => case10 (pre, S_PSHUFW op1 op2 imm)
+                     | MASKMOVQ op1 op2 => case10 (pre, S_MASKMOVQ op1 op2)
+                     | MOVNTPS op1 op2 => case10 (pre, S_MOVNTPS op1 op2)
+                     | MOVNTQ op1 op2 => case10 (pre, S_MOVNTQ op1 op2)
+                     | PREFETCHT0 op => case10 (pre, S_PREFETCHT0 op)
+                     | PREFETCHT1 op => case10 (pre, S_PREFETCHT1 op)
+                     | PREFETCHT2 op => case10 (pre, S_PREFETCHT2 op)
+                     | PREFETCHNTA op => case10 (pre, S_PREFETCHNTA op)
+                     | SFENCE => case10 (pre, S_SFENCE)
+
+                     (* | _ => None *)
+                   end)
+               & _); clear_ast_defs;
+    unfold invertible; split; [unfold printable | unfold parsable]; 
+    compute [snd fst]; intros.
+    - destruct_union; destruct v as [pre hi];
+        abstract (destruct hi; printable_tac).
+    - Time abstract (destruct w as [pre i]; destruct i; parsable_tac).
+  Defined.
+
+
 
 
   (* Definition instr_grammars_seg_override :=  *)
@@ -5579,6 +7263,8 @@ End X86_PARSER_ARG.
       +++
     (ast_env_cat prefix_grammar_seg_override
        instr_grammars_seg_override).
+
+
 
   Definition instr_grammar_env : AST_Env (pair_t prefix_t instruction_t).
     let ige := eval cbv beta
