x86model/Model/ParserArg.v
@@ -47,6 +47,358 @@ Module X86_PARSER_ARG.
   Require Import X86Syntax.
   Require Import Bits.
   Local Open Scope Z_scope.
+
+  (** Hierarchical instruction syntax. The problem with a parser mapping
+      directly to instr is that the current instr syntax is flat with more
+      than 350 cases. A bidirectional grammar for instr would need to
+      construct an AST with many cases and Coq runs out of mem during the
+      proof search (even with the help of the abstract tactical).
+   
+      So we introduce an hierarhical instruction syntax as an intermiary for
+      coping with the scability issue.
+   *)
+
+  (** This set of integer instructions
+     - take no parameters
+     - take only the seg_override prefix *)
+  Inductive i_instr1 : Set :=
+  | I_AAA
+  | I_AAD 
+  | I_AAM 
+  | I_AAS 
+  | I_CLC 
+  | I_CLD 
+  | I_CLI 
+  | I_CLTS 
+  | I_CMC
+  | I_CPUID 
+  | I_DAA 
+  | I_DAS
+  | I_HLT  
+  | I_INT
+  | I_INTO
+  | I_INVD
+  | I_IRET
+  | I_LAHF
+  | I_LEAVE
+  | I_POPA 
+  | I_POPF
+  | I_PUSHA
+  | I_PUSHF
+  | I_RDMSR
+  | I_RDPMC
+  | I_RDTSC
+  | I_RDTSCP
+  | I_RSM
+  | I_SAHF
+  | I_STC
+  | I_STD
+  | I_STI
+  | I_UD2
+  | I_WBINVD
+  | I_WRMSR
+  | I_XLAT.
+
+  (** This set of integer instructions
+     - take some parameters
+     - take only the seg_override prefix
+     - first letter of name in A-L *)
+  Inductive i_instr2 : Set :=
+  | I_ARPL (op1 op2:operand)
+  | I_BOUND (op1 op2:operand)
+  | I_BSF (op1 op2:operand)
+  | I_BSR (op1 op2:operand)
+  | I_BSWAP (r:register)
+  | I_BT (op1 op2:operand)
+  | I_CALL (near:bool)(absolute: bool)(op1:operand)(sel:option selector)
+  | I_IN (w:bool)(p: option port_number)
+  | I_INTn (it:interrupt_type)
+  | I_INVLPG (op1:operand)
+  | I_Jcc (ct:condition_type)(disp:int32)
+  | I_JCXZ (b:int8)
+  | I_JMP (near:bool)(absolute:bool)(op1: operand)(sel:option selector)
+  | I_LAR (op1 op2:operand)
+  | I_LDS (op1 op2:operand)
+  | I_LEA (op1 op2:operand)
+  | I_LES (op1 op2:operand)
+  | I_LFS (op1 op2:operand)
+  | I_LGDT (op1:operand)
+  | I_LGS (op1 op2:operand)
+  | I_LIDT (op1:operand)
+  | I_LLDT (op1:operand)
+  | I_LMSW (op1:operand)
+  | I_LOOP (disp:int8)
+  | I_LOOPZ (disp:int8)
+  | I_LOOPNZ (disp:int8)
+  | I_LSL  (op1 op2:operand)
+  | I_LSS (op1 op2:operand)
+  | I_LTR (op1:operand).
+
+  (** This set of integer instructions
+     - take some parameters
+     - take only the seg_override prefix
+     - first letter of name in M-Z *)
+  Inductive i_instr3 : Set :=
+  | I_MOVCR (direction:bool)(cr:control_register)(r:register)
+  | I_MOVDR (direction:bool)(dr:debug_register)(r:register)
+  | I_MOVSR (direction:bool)(sr:segment_register)(op1:operand)
+  | I_MOVBE (op1 op2:operand)
+  | I_OUT (w:bool)(p:option port_number)
+  | I_POP (op1:operand)
+  | I_POPSR (sr:segment_register)
+  | I_PUSH (w:bool)(op1:operand)
+  | I_PUSHSR (sr:segment_register)
+  | I_RCL (w:bool)(op1:operand)(ri:reg_or_immed)
+  | I_RCR (w:bool)(op1:operand)(ri:reg_or_immed)
+  | I_SETcc (ct:condition_type)(op1:operand)
+  | I_SGDT (op1:operand)
+  | I_SIDT (op1:operand)
+  | I_SLDT (op1:operand)
+  | I_SMSW (op1:operand)
+  | I_STR (op1:operand)
+  | I_VERR (op1:operand)
+  | I_VERW (op1:operand).
+
+  (** These integer instructions can take prefixes in prefix_grammar_rep, 
+      or prefix_grammar_repn. *)
+  Inductive i_instr4 : Set :=
+  (* the following can take prefixes in prefix_grammar_rep *)
+  | I_INS (w:bool)
+  | I_OUTS (w:bool)
+  | I_MOVS (w:bool)
+  | I_LODS (w:bool)
+  | I_STOS (w:bool)
+  | I_RET (same_segment:bool)(disp:option int16)
+  (* the following can take prefixes in prefix_grammar_repn *)
+  | I_CMPS (w:bool)
+  | I_SCAS (w:bool).
+
+  (** This set of instructions can take prefixes in 
+      prefix_grammar_seg_with_op_override, prefix_grammar_lock_no_op_override,
+      or prefix_grammar_lock_with_op_override *)
+  Inductive i_instr5 : Set := 
+  | I_ADC (w:bool)(op1 op2:operand)
+  | I_ADD (w:bool)(op1 op2:operand)
+  | I_AND (w:bool)(op1 op2:operand)
+  | I_BTC (op1 op2:operand)
+  | I_BTR (op1 op2:operand)
+  | I_BTS (op1 op2:operand)
+  | I_CMP (w:bool)(op1 op2:operand)
+  | I_CMPXCHG (w:bool)(op1 op2:operand)
+  | I_DEC (w:bool)(op1:operand)
+  | I_IMUL (w:bool)(op1:operand) (opopt: option operand) (iopt:option int32)
+  | I_INC (w:bool)(op1:operand)
+  | I_MOV (w:bool)(op1 op2:operand)
+  | I_NEG (w:bool)(op:operand)
+  | I_NOT (w:bool)(op:operand)
+  | I_OR (w:bool)(op1 op2:operand)
+  | I_SBB (w:bool)(op1 op2:operand)
+  | I_SUB (w:bool)(op1 op2:operand)
+  | I_TEST (w:bool)(op1 op2:operand)
+  | I_XADD (w:bool)(op1 op2:operand)
+  | I_XCHG (w:bool)(op1 op2:operand)
+  | I_XOR (w:bool)(op1 op2:operand).
+
+  (** this set of instructions can take prefixes in prefix_grammar_seg_op_override *)
+  Inductive i_instr6 : Set := 
+  | I_CDQ 
+  | I_CMOVcc (ct:condition_type)(op1 op2: operand)
+  | I_CWDE 
+  | I_DIV (w:bool)(op1:operand)
+  | I_IDIV (w:bool)(op1:operand)
+  | I_MOVSX (w:bool)(op1 op2:operand)
+  | I_MOVZX (w:bool)(op1 op2:operand)
+  | I_MUL (w:bool)(op1:operand)
+  | I_NOP (op:operand)
+  | I_ROL (w:bool)(op1:operand)(ri:reg_or_immed)
+  | I_ROR (w:bool)(op1:operand)(ri:reg_or_immed)
+  | I_SAR (w:bool)(op1:operand)(ri:reg_or_immed)
+  | I_SHL (w:bool)(op1:operand)(ri:reg_or_immed)
+  | I_SHLD (op1:operand)(r:register)(ri:reg_or_immed)
+  | I_SHR (w:bool)(op1:operand)(ri:reg_or_immed)
+  | I_SHRD (op1:operand)(r:register)(ri:reg_or_immed).
+
+  (** the first set of floating-point instrs *)
+  Inductive f_instr1 : Set :=
+  | F_F2XM1
+  | F_FABS
+  | F_FADD (zerod: bool) (op1: fp_operand)
+  | F_FADDP (op1: fp_operand)
+  | F_FBLD (op1: fp_operand)
+  | F_FBSTP (op1: fp_operand)
+  | F_FCHS
+  | F_FCMOVcc (ct:fp_condition_type)(op1: fp_operand)
+  | F_FCOM (op1: fp_operand)
+  | F_FCOMP (op1: fp_operand)
+  | F_FCOMPP
+  | F_FCOMIP (op1: fp_operand)
+  | F_FCOS
+  | F_FDECSTP
+  | F_FDIV (zerod: bool) (op: fp_operand)
+  | F_FDIVP (op1: fp_operand)
+  | F_FDIVR (zerod: bool) (op: fp_operand)
+  | F_FDIVRP (op1: fp_operand)
+  | F_FFREE (op1: fp_operand)
+  | F_FIADD (op1: fp_operand)
+  | F_FICOM (op1: fp_operand)
+  | F_FICOMP (op1: fp_operand)
+  | F_FIDIV (op1: fp_operand)
+  | F_FIDIVR (op1: fp_operand)
+  | F_FILD (op1: fp_operand)
+  | F_FIMUL (op1: fp_operand)
+  | F_FINCSTP
+  | F_FIST (op1: fp_operand)
+  | F_FISTP (op1: fp_operand)
+  | F_FISUB (op1: fp_operand)
+  | F_FISUBR (op1: fp_operand)
+  | F_FLD (op1: fp_operand)
+  | F_FLD1
+  | F_FLDCW (op1: fp_operand)
+  | F_FLDENV (op1: fp_operand)
+  | F_FLDL2E
+  | F_FLDL2T
+  | F_FLDLG2
+  | F_FLDLN2
+  | F_FLDPI
+  | F_FLDZ
+  | F_FMUL (zerod: bool) (op1: fp_operand)
+  | F_FMULP (op1: fp_operand).
+
+  Inductive f_instr2 : Set :=
+  | F_FNCLEX
+  | F_FNINIT
+  | F_FNOP
+  | F_FNSAVE (op1: fp_operand)
+  | F_FNSTCW (op1 : fp_operand)
+  | F_FNSTSW (op1 : option fp_operand)
+  | F_FPATAN
+  | F_FPREM
+  | F_FPREM1
+  | F_FPTAN
+  | F_FRNDINT
+  | F_FRSTOR (op1: fp_operand)
+  | F_FSCALE
+  | F_FSIN
+  | F_FSINCOS
+  | F_FSQRT
+  | F_FST (op1: fp_operand)
+  | F_FSTENV (op1: fp_operand)
+  | F_FSTP (op1: fp_operand)
+  | F_FSUB (zerod: bool) (op: fp_operand)
+  | F_FSUBP (op1: fp_operand)
+  | F_FSUBR (zerod: bool) (op: fp_operand)
+  | F_FSUBRP (op1: fp_operand)
+  | F_FTST
+  | F_FUCOM (op1: fp_operand)
+  | F_FUCOMP (op1: fp_operand)
+  | F_FUCOMPP
+  | F_FUCOMI (op1: fp_operand)
+  | F_FUCOMIP (op1: fp_operand)
+  | F_FXAM
+  | F_FXCH (op1: fp_operand)
+  | F_FXTRACT
+  | F_FYL2X
+  | F_FYL2XP1
+  | F_FWAIT.
+
+  (** mmx instructions *)
+  Inductive m_instr : Set :=
+  | M_EMMS
+  | M_MOVD (op1 op2: mmx_operand)
+  | M_MOVQ (op1 op2: mmx_operand)
+  | M_PACKSSDW (op1 op2: mmx_operand)
+  | M_PACKSSWB (op1 op2: mmx_operand)
+  | M_PACKUSWB (op1 op2: mmx_operand)
+  | M_PADD (gg:mmx_granularity) (op1 op2: mmx_operand)
+  | M_PADDS (gg:mmx_granularity) (op1 op2: mmx_operand)
+  | M_PADDUS (gg:mmx_granularity) (op1 op2: mmx_operand)
+  | M_PAND (op1 op2 : mmx_operand)
+  | M_PANDN (op1 op2 : mmx_operand)
+  | M_PCMPEQ (gg:mmx_granularity) (op1 op2 : mmx_operand)
+  | M_PCMPGT (gg:mmx_granularity) (op1 op2 : mmx_operand)
+  | M_PMADDWD (op1 op2 : mmx_operand)
+  | M_PMULHUW (op1 op2 : mmx_operand)
+  | M_PMULHW (op1 op2 : mmx_operand)
+  | M_PMULLW (op1 op2 : mmx_operand)
+  | M_POR (op1 op2 : mmx_operand)
+  | M_PSLL (gg:mmx_granularity) (op1 op2: mmx_operand)
+  | M_PSRA (gg:mmx_granularity) (op1 op2: mmx_operand)
+  | M_PSRL (gg:mmx_granularity) (op1 op2: mmx_operand)
+  | M_PSUB (gg:mmx_granularity) (op1 op2: mmx_operand)
+  | M_PSUBS (gg:mmx_granularity) (op1 op2: mmx_operand)
+  | M_PSUBUS (gg:mmx_granularity) (op1 op2: mmx_operand)
+  | M_PUNPCKH (gg:mmx_granularity) (op1 op2: mmx_operand)
+  | M_PUNPCKL (gg:mmx_granularity) (op1 op2: mmx_operand)
+  | M_PXOR (op1 op2 : mmx_operand).
+
+  (** sse instructions *)
+  Inductive s_instr1 : Set :=
+  | S_ADDPS (op1 op2: sse_operand)
+  | S_ADDSS (op1 op2: sse_operand)
+  | S_ANDNPS (op1 op2: sse_operand)
+  | S_ANDPS (op1 op2: sse_operand)
+  | S_CMPPS (op1 op2:sse_operand) (imm:int8)
+  | S_CMPSS (op1 op2: sse_operand) (imm:int8)
+  | S_COMISS (op1 op2: sse_operand)
+  | S_CVTPI2PS (op1 op2: sse_operand)
+  | S_CVTPS2PI (op1 op2: sse_operand)
+  | S_CVTSI2SS (op1 op2: sse_operand)
+  | S_CVTSS2SI (op1 op2: sse_operand)
+  | S_CVTTPS2PI (op1 op2: sse_operand)
+  | S_CVTTSS2SI (op1 op2: sse_operand)
+  | S_DIVPS (op1 op2: sse_operand)
+  | S_DIVSS (op1 op2: sse_operand)
+  | S_LDMXCSR (op1: sse_operand)
+  | S_MAXPS (op1 op2: sse_operand)
+  | S_MAXSS (op1 op2: sse_operand)
+  | S_MINPS (op1 op2: sse_operand)
+  | S_MINSS (op1 op2: sse_operand)
+  | S_MOVAPS (op1 op2: sse_operand)
+  | S_MOVHLPS (op1 op2: sse_operand)
+  | S_MOVHPS (op1 op2: sse_operand)
+  | S_MOVLHPS (op1 op2: sse_operand)
+  | S_MOVLPS (op1 op2: sse_operand)
+  | S_MOVMSKPS (op1 op2: sse_operand)
+  | S_MOVSS (op1 op2: sse_operand)
+  | S_MOVUPS (op1 op2: sse_operand)
+  | S_MULPS (op1 op2: sse_operand)
+  | S_MULSS (op1 op2: sse_operand)
+  | S_ORPS (op1 op2: sse_operand)
+  | S_RCPPS (op1 op2: sse_operand)
+  | S_RCPSS (op1 op2: sse_operand)
+  | S_RSQRTPS (op1 op2: sse_operand)
+  | S_RSQRTSS (op1 op2: sse_operand).
+
+  Inductive s_instr2 : Set :=
+  | S_SHUFPS (op1 op2: sse_operand) (imm:int8)
+  | S_SQRTPS (op1 op2: sse_operand)
+  | S_SQRTSS (op1 op2: sse_operand)
+  | S_STMXCSR (op1 : sse_operand)
+  | S_SUBPS (op1 op2: sse_operand)
+  | S_SUBSS (op1 op2: sse_operand)
+  | S_UCOMISS (op1 op2: sse_operand)
+  | S_UNPCKHPS (op1 op2: sse_operand)
+  | S_UNPCKLPS (op1 op2: sse_operand)
+  | S_XORPS (op1 op2: sse_operand)
+  | S_PAVGB (op1 op2: sse_operand)
+  | S_PEXTRW (op1 op2: sse_operand) (imm:int8)
+  | S_PINSRW (op1 op2: sse_operand) (imm:int8)
+  | S_PMAXSW (op1 op2: sse_operand)
+  | S_PMAXUB (op1 op2: sse_operand)
+  | S_PMINSW (op1 op2: sse_operand)
+  | S_PMINUB (op1 op2: sse_operand)
+  | S_PMOVMSKB (op1 op2: sse_operand)
+  | S_PSADBW (op1 op2: sse_operand)
+  | S_PSHUFW (op1 op2: sse_operand) (imm:int8)
+  | S_MASKMOVQ (op1 op2: sse_operand)
+  | S_MOVNTPS (op1 op2: sse_operand)
+  | S_MOVNTQ (op1 op2: sse_operand)
+  | S_PREFETCHT0 (op1: sse_operand)
+  | S_PREFETCHT1 (op1: sse_operand)
+  | S_PREFETCHT2 (op1: sse_operand)
+  | S_PREFETCHNTA (op1: sse_operand)
+  | S_SFENCE.
+
   
   Definition char_p : Set := bool.
   Definition char_dec : forall (c1 c2:char_p), {c1=c2}+{c1<>c2} := bool_dec.
@@ -65,6 +417,17 @@ Module X86_PARSER_ARG.
   | MMX_Granularity_t : type
   | MMX_Operand_t : type
   | SSE_Operand_t : type
+  | I_Instr1_t
+  | I_Instr2_t
+  | I_Instr3_t
+  | I_Instr4_t
+  | I_Instr5_t
+  | I_Instr6_t
+  | F_Instr1_t
+  | F_Instr2_t
+  | M_Instr_t
+  | S_Instr1_t
+  | S_Instr2_t
   | Instruction_t : type
   | Control_Register_t : type
   | Debug_Register_t : type
@@ -109,6 +472,17 @@ Module X86_PARSER_ARG.
       | MMX_Operand_t => mmx_operand
       | SSE_Operand_t => sse_operand
       | Instruction_t => instr
+      | I_Instr1_t => i_instr1
+      | I_Instr2_t => i_instr2
+      | I_Instr3_t => i_instr3
+      | I_Instr4_t => i_instr4
+      | I_Instr5_t => i_instr5
+      | I_Instr6_t => i_instr6
+      | F_Instr1_t => f_instr1
+      | F_Instr2_t => f_instr2
+      | M_Instr_t => m_instr
+      | S_Instr1_t => s_instr1
+      | S_Instr2_t => s_instr2
       | Control_Register_t => control_register
       | Debug_Register_t => debug_register
       | Segment_Register_t => segment_register
